pre build merge

generic/Zeta.Generic.Thread.fst
@@ -68,6 +68,27 @@ let add_seq (#vspec:_) (ep: epoch) (tl: verifiable_log vspec)
   = let fm = IF.to_fm (is_blum_add_epoch_ifn #vspec ep) (blum_add_elem_ifn #vspec) in
     IF.filter_map fm tl
 
+let add_seq_empty (#vspec:_) (ep: epoch) (tl: verifiable_log vspec)
+  : Lemma (ensures (length tl = 0 ==> S.length (add_seq ep tl) = 0))
+  = if length tl = 0 then ()
+
+let add_seq_snoc
+  (#vspec:_)
+  (ep: epoch)
+  (tl: verifiable_log vspec {length tl > 0})
+  : Lemma (ensures (let i = length tl - 1 in
+                    let tl' = prefix tl i in
+                    let as' = add_seq ep tl' in
+                    let as = add_seq ep tl in
+                    if is_blum_add_ep ep tl i then
+                      as == SA.append1 as' (blum_add_elem tl i)
+                    else
+                      as == as'))
+  = let fm = IF.to_fm (is_blum_add_epoch_ifn #vspec ep) (blum_add_elem_ifn #vspec) in
+    let i = length tl - 1 in
+    if is_blum_add_ep ep tl i then
+      IF.lemma_filter_map_snoc fm tl
+
 let add_seq_map (#vspec:_) (tl: verifiable_log vspec) (i: seq_index tl {is_blum_add tl i})
   : (let be = blum_add_elem tl i in
      let ep = be.t.e in
@@ -143,6 +164,31 @@ let evict_seq (#vspec:_) (ep: epoch) (tl: verifiable_log vspec)
   : S.seq (ms_hashfn_dom vspec.app)
   = let fm = IF.to_fm (is_blum_evict_epoch_ifn #vspec ep) (blum_evict_elem_ifn #vspec) in
     IF.filter_map fm tl
+
+let evict_seq_empty (#vspec:_) (ep: epoch) (tl: verifiable_log vspec)
+  : Lemma (ensures (length tl = 0 ==> S.length (evict_seq ep tl) = 0))
+  = if length tl = 0 then ()
+
+let evict_seq_snoc
+  (#vspec:_)
+  (ep: epoch)
+  (tl: verifiable_log vspec {length tl > 0})
+  : Lemma (ensures (let i = length tl - 1 in
+                    let tl' = prefix tl i in
+                    let es' = evict_seq ep tl' in
+                    let es = evict_seq ep tl in
+                    if is_blum_evict_ep ep tl i then
+                      es == SA.append1 es' (blum_evict_elem tl i)
+                    else
+                      es == es'))
+  = let fm = IF.to_fm (is_blum_evict_epoch_ifn #vspec ep) (blum_evict_elem_ifn #vspec) in
+    let i = length tl - 1 in
+    let tl' = prefix tl i in
+    let es' = evict_seq ep tl' in
+    let es = evict_seq ep tl in
+
+    if is_blum_evict_ep ep tl i then
+      IF.lemma_filter_map_snoc fm tl
 
 let evict_seq_map (#vspec:_) (tl: verifiable_log vspec) (i: seq_index tl {is_blum_evict tl i})
   : (let be = blum_evict_elem tl i in
@@ -289,6 +335,24 @@ let app_fcrs_within_ep
   : S.seq (appfn_call_res vspec.app)
   = let fm = IF.to_fm (is_appfn_within_ep_ifn #vspec ep) (to_app_fcr #vspec) in
     IF.filter_map fm tl
+
+let app_fcrs_empty (#vspec:_) (ep: epoch) (tl: verifiable_log vspec)
+  : Lemma (ensures (length tl = 0 ==> S.length (app_fcrs_within_ep ep tl) = 0))
+  = ()
+
+let app_fcrs_snoc (#vspec:_) (ep: epoch) (tl: verifiable_log vspec {length tl > 0})
+  : Lemma (ensures (let i = length tl - 1 in
+                    let tl' = prefix tl i in
+                    let fcrs' = app_fcrs_within_ep ep tl' in
+                    let fcrs = app_fcrs_within_ep ep tl in
+                    if is_appfn_within_epoch ep tl i then
+                      fcrs == SA.append1 fcrs' (to_app_fcr tl i)
+                    else
+                      fcrs == fcrs'))
+  = let fm = IF.to_fm (is_appfn_within_ep_ifn #vspec ep) (to_app_fcr #vspec) in
+    let i = length tl - 1 in
+    if is_appfn_within_epoch ep tl i then
+      IF.lemma_filter_map_snoc fm tl
 
 let app_fcrs_ep_map (#vspec:_)
     (ep: epoch)
