utils/Zeta.MultiSet.SSeq.fsti
@@ -7,9 +7,29 @@ open Zeta.SSeq
 open Zeta.MultiSet
 open Zeta.Interleave
 
+module S = FStar.Seq
+module SA = Zeta.SeqAux
+
 /// Construct a multiset from a seq of sequences
 
 val sseq2mset (#a:eqtype) (#f:cmp a) (s:sseq a) : mset a f
 
 val lemma_interleaving_multiset (#a:_) (#f:cmp a) (#n:_) (il: interleaving a n)
   : Lemma (ensures (seq2mset #_ #f (i_seq il) == sseq2mset (s_seq il)))
+
+val union_all (#a:eqtype) (#f: cmp a) (s: S.seq (mset a f))
+  : mset a f
+
+val union_all_empty (#a: eqtype) (#f: cmp a) (s: S.seq (mset a f){ S.length s = 0 })
+  : Lemma (ensures (union_all s == empty #a #f))
+
+val union_all_cons (#a: eqtype) (#f: cmp a) (s: Seq.seq (mset a f) {Seq.length s > 0})
+  : Lemma (ensures (let tail = Seq.tail s in
+                    let hd = Seq.head s in
+                    union_all s == union hd (union_all tail)))
+
+val union_all_sseq (#a: eqtype) (#f: cmp a) (s: sseq a)
+  : Lemma (ensures (let ms1: mset a f = sseq2mset s in
+                    let sms = S.init (S.length s) (fun i -> seq2mset (S.index s i)) in
+                    let ms2: mset a f = union_all sms in
+                    ms1 == ms2))
