steel/Zeta.Steel.AddMRel.fsti
@@ -1,0 +1,285 @@
+module Zeta.Steel.AddMRel
+
+open Zeta.Steel.KeyUtils
+open Zeta.Steel.ThreadStateModel
+open Zeta.Steel.Rel
+open Zeta.Steel.StoreRel
+open Zeta.Steel.ThreadRelDef
+
+module T = Zeta.Steel.FormatsManual
+module SS = Zeta.Steel.StoreRel
+module IV = Zeta.Intermediate.Verifier
+
+(* steel-level addm param *)
+noeq type addm_param =
+  | AMP: s: s_slot_id ->
+          p: payload ->
+          s': s_slot_id ->
+          vs': s_thread_state -> addm_param
+
+let addm_precond0 (a: addm_param)
+  = match a with
+    | AMP s p s' _ ->
+    check_slot_bounds s /\
+    check_slot_bounds s' /\
+    Some? (record_of_payload p)
+
+(* the key being added *)
+let addm_key (a: addm_param {addm_precond0 a})
+  = match a with
+    | AMP _ p _ _ -> match record_of_payload p with
+                     | Some (| gk, gv |) -> gk
+
+let addm_base_key (a: addm_param {addm_precond0 a})
+  = to_base_key (addm_key a)
+
+(* slot where the record is being added *)
+let addm_slot (a: addm_param) =
+  match a with
+  | AMP s _ _ _ -> s
+
+(* the slot where the ancestore record is stored *)
+let addm_anc_slot (a: addm_param) =
+  match a with
+  | AMP _ _ s' _ -> s'
+
+(* the state of the store before the add *)
+let addm_store_pre (a: addm_param) =
+  match a with
+  | AMP _ _ _ vs' ->  vs'.store
+
+(* initial set of addm preconditions: vaddm fails if these are not met *)
+let addm_precond1 (a: addm_param) =
+  let st' = addm_store_pre a in
+  let s = addm_slot a in
+  let s' = addm_anc_slot a in
+  addm_precond0 a /\
+  s <> s' /\
+  inuse_slot st' s' /\
+  empty_slot st' s /\
+  (let k' = stored_base_key st' s' in
+   let gk = addm_key a in
+   is_proper_descendent (to_base_key gk) k')
+
+let addm_value_pre (a: addm_param {addm_precond1 a})  =
+  match a with
+  | AMP _ p _ _ -> match record_of_payload p with
+                   | Some (| gk, gv |) -> gv
+
+let addm_hash_val_pre (a: addm_param {addm_precond1 a}) =
+  hashfn (addm_value_pre a)
+
+let addm_anc_key (a: addm_param {addm_precond1 a}): GTot (T.internal_key) =
+  stored_base_key (addm_store_pre a) (addm_anc_slot a)
+
+let addm_anc_val_pre (a: addm_param {addm_precond1 a}) =
+  let st' = addm_store_pre a in
+  let s' = addm_anc_slot a in
+  let Some mv = to_merkle_value (stored_value st' s') in
+  mv
+
+let addm_dir (a: addm_param {addm_precond1 a}) =
+  desc_dir (addm_base_key a) (addm_anc_key a)
+
+let mv_points_to_none (mv: T.mval_value) (d: bool)
+  = desc_hash_dir mv d = T.Dh_vnone ()
+
+let mv_points_to_some (v:T.mval_value) (d:bool): bool =
+  T.Dh_vsome? (desc_hash_dir v d)
+
+let mv_pointed_key (v:T.mval_value) (d: bool{mv_points_to_some v d}): T.base_key =
+  let T.Dh_vsome dh = desc_hash_dir v d in
+  dh.dhd_key
+
+let mv_pointed_hash (v:T.mval_value) (d: bool{mv_points_to_some v d}): T.hash_value =
+  let T.Dh_vsome dh = desc_hash_dir v d in
+  dh.dhd_h
+
+let mv_points_to (v:T.mval_value) (d:bool) (k:T.base_key): bool =
+  mv_points_to_some v d && mv_pointed_key v d = k
+
+let mv_evicted_to_blum (v: T.mval_value) (d: bool {mv_points_to_some v d})
+  = let T.Dh_vsome dh = desc_hash_dir v d in
+    dh.evicted_to_blum = T.Vtrue
+
+let addm_precond2 (a: addm_param) =
+  addm_precond1 a /\
+  (let mv' = addm_anc_val_pre a in
+   let d = addm_dir a in
+   mv_points_to_none mv' d \/                          // case A: ancestor points to nothing along d
+   mv_points_to mv' d (addm_base_key a) \/                  // case B: ancestor points to key being added
+   is_proper_descendent (mv_pointed_key mv' d) (addm_base_key a)) // case C: ancestor points to some key below key being added
+
+// case A:
+let addm_anc_points_null (a: addm_param {addm_precond2 a}) =
+  mv_points_to_none (addm_anc_val_pre a) (addm_dir a)
+
+// case B:
+let addm_anc_points_to_key (a: addm_param {addm_precond2 a}) =
+  mv_points_to (addm_anc_val_pre a) (addm_dir a) (addm_base_key a)
+
+// desc hash at ancestor along addm direction
+let addm_desc_hash_dir (a: addm_param {addm_precond2 a /\ addm_anc_points_to_key a}) =
+  desc_hash_dir (addm_anc_val_pre a) (addm_dir a)
+
+// case C:
+let addm_anc_points_to_desc (a: addm_param {addm_precond2 a}) =
+  let mv' = addm_anc_val_pre a in
+  let d = addm_dir a in
+  mv_points_to_some mv' d /\
+  is_proper_descendent (mv_pointed_key mv' d) (addm_base_key a)
+
+// desc key for case C:
+let addm_desc (a:addm_param {addm_precond2 a /\ addm_anc_points_to_desc a}):
+  GTot (k2: T.base_key {is_proper_descendent k2 (addm_base_key a)}) =
+  mv_pointed_key (addm_anc_val_pre a) (addm_dir a)
+
+let addm_desc_dir (a: addm_param {addm_precond2 a /\ addm_anc_points_to_desc a})
+  : GTot bool
+  = desc_dir (addm_desc a) (addm_base_key a)
+
+let addm_precond (a: addm_param) =
+  let st = addm_store_pre a in
+  let s' = addm_anc_slot a in
+  addm_precond2 a /\
+  (let d = addm_dir a in
+   (addm_anc_points_null a ==> (addm_value_pre a = init_value (addm_key a) /\
+                              points_to_none st s' d)) /\
+   (addm_anc_points_to_key a ==> (addm_desc_hash_dir a = T.Dh_vsome ({ dhd_key = (addm_base_key a);
+                                                                    dhd_h = (addm_hash_val_pre a);
+                                                                    evicted_to_blum = T.Vfalse })) /\
+                                points_to_none st s' d) /\
+   (addm_anc_points_to_desc a ==> (addm_value_pre a = init_value (addm_key a))))
+
+(* does the ancestor point to the descendant slot *)
+let addm_has_desc_slot (a: addm_param {addm_precond a}) =
+  addm_anc_points_to_desc a /\
+  (let s' = addm_anc_slot a in
+   let st' = addm_store_pre a in
+   let d = addm_dir a in
+   SS.points_to_some_slot st' s' d)
+
+let addm_desc_slot (a: addm_param {addm_precond a /\ addm_has_desc_slot a}) =
+  let s' = addm_anc_slot a in
+  let st' = addm_store_pre a in
+  let d = addm_dir a in
+  pointed_slot st' s' d
+
+let addm_value_postcond (a: addm_param {addm_precond a})
+  (v: T.value {is_value_of (addm_key a) v}) =
+  (addm_anc_points_null a /\ (v = addm_value_pre a)) \/
+  (addm_anc_points_to_key a /\ (v = addm_value_pre a)) \/
+  (addm_anc_points_to_desc a /\
+    (let dd = addm_desc_dir a in
+     let odd = not dd in
+     let Some mv = to_merkle_value v in
+     desc_hash_dir mv dd = desc_hash_dir (addm_anc_val_pre a) (addm_dir a) /\
+     desc_hash_dir mv odd = T.Dh_vnone ()))
+
+let addm_slot_points_postcond (a: addm_param {addm_precond a}) (st: contents) =
+  let s = addm_slot a in
+  let st' = addm_store_pre a in
+  let s' = addm_anc_slot a in
+  let d = addm_dir a in
+  inuse_slot st s /\
+  ((addm_anc_points_null a /\ points_to_none st s true /\ points_to_none st s false) \/
+   (addm_anc_points_to_key a /\ points_to_none st s true /\ points_to_none st s false) \/
+   (addm_anc_points_to_desc a /\ (points_to_info st s (addm_desc_dir a) = points_to_info st' s' d) /\
+                                 points_to_none st s (not (addm_desc_dir a))))
+
+(* post-condition on addm slot *)
+let addm_slot_postcond (a: addm_param {addm_precond a}) (st: contents) =
+  let s = addm_slot a in
+  inuse_slot st s  /\                          // in use
+  stored_key st s = addm_key a   /\            // stores key k
+  add_method_of st s = MAdd /\            // stores the correct add method
+  addm_value_postcond a (stored_value st s) /\ // value postcond
+  addm_slot_points_postcond a st /\
+  has_parent st s /\
+  parent_slot st s = addm_anc_slot a /\
+  parent_dir st s = addm_dir a
+
+let addm_anc_val_postcond (a: addm_param {addm_precond a}) (mv: T.mval_value) =
+  let mv' = addm_anc_val_pre a in
+  let d = addm_dir a in
+  let od = not d in
+  desc_hash_dir mv od = desc_hash_dir mv' od /\               // merkle value unchanged in other direction
+  mv_points_to mv d (addm_base_key a) /\          // merkle value points to k in addm direction
+  mv_evicted_to_blum mv d = false /\
+  mv_pointed_hash mv d =
+    (if (addm_anc_points_to_key a) then
+      mv_pointed_hash mv' d
+    else
+      zero)
+
+let addm_anc_slot_points_postcond (a: addm_param {addm_precond a}) (st: contents) =
+  let st' = addm_store_pre a in
+  let s' = addm_anc_slot a in
+  let d = addm_dir a in
+  let od = not d in
+  inuse_slot st s' /\
+  points_to_info st s' od = points_to_info st' s' od /\        // points to does not change in other dir
+  points_to_dir st s' d (addm_slot a)
+
+let addm_anc_slot_postcond (a: addm_param {addm_precond a}) (st: contents) =
+  let s' = addm_anc_slot a in
+  let st' = addm_store_pre a in
+  inuse_slot st s' /\
+  stored_base_key st s' = addm_anc_key a /\
+  add_method_of st s' = add_method_of st' s' /\
+  addm_anc_val_postcond a (Some?. v (to_merkle_value (stored_value st s'))) /\
+  addm_anc_slot_points_postcond a st /\
+  (let Some e' = get_slot st' s' in
+   let Some e = get_slot st s' in
+   e.parent_slot = e'.parent_slot)
+
+let addm_desc_slot_postcond (a: addm_param {addm_precond a /\ addm_has_desc_slot a}) (st: contents) =
+  let sd = addm_desc_slot a in
+  let st' = addm_store_pre a in
+  inuse_slot st sd /\ inuse_slot st' sd /\
+  stored_key st sd = stored_key st' sd /\
+  stored_value st sd = stored_value st' sd /\
+  add_method_of st sd = add_method_of st' sd /\
+  has_parent st sd /\
+  parent_slot st sd = addm_slot a /\
+  parent_dir st sd = addm_desc_dir a /\
+  points_to_info st sd true = points_to_info st' sd true /\
+  points_to_info st sd false = points_to_info st' sd false
+
+let addm_postcond (a: addm_param {addm_precond a}) (vs: s_thread_state) =
+  let vs' = a.vs' in
+
+  (vs.failed = vs'.failed /\
+   vs.thread_id = vs'.thread_id /\ vs.clock = vs'.clock /\                // everything except store is unchanged
+   (addm_has_desc_slot a /\
+    identical_except3 vs.store vs'.store (addm_slot a) (addm_anc_slot a) (addm_desc_slot a) /\
+    addm_desc_slot_postcond a vs.store
+    \/
+    ~ (addm_has_desc_slot a) /\
+    identical_except2 vs.store vs'.store (addm_slot a) (addm_anc_slot a)) /\
+   addm_slot_postcond a vs.store /\                                      // postcond on slot s
+   addm_anc_slot_postcond a vs.store)                                    // postcond on slot s'
+
+let i_addm_param = IV.addm_param i_vcfg
+
+let related_addm_param (a: addm_param) (i_a: i_addm_param)
+  = let AMP _ _ _ tsm = a in
+    let IV.AMP _ _ _ i_tsm = i_a in
+    addm_precond0 a /\
+    related_slot (addm_slot a) (IV.addm_slot i_a) /\
+    related_slot (addm_anc_slot a) (IV.addm_anc_slot i_a) /\
+    related_tsm tsm i_tsm /\
+    related_key (addm_key a) (IV.addm_key i_a) /\
+    (addm_precond1 a ==> IV.addm_precond1 i_a ==>
+     related_val (addm_value_pre a)  (IV.addm_value_pre i_a))
+
+val related_addm_precond (a: addm_param) (i_a: i_addm_param)
+  : Lemma (requires (related_addm_param a i_a /\ addm_precond a))
+          (ensures (IV.addm_precond i_a))
+          [SMTPat (related_addm_param a i_a)]
+
+val related_addm_postcond (a: addm_param) (i_a: i_addm_param) (tsm_: s_thread_state) (i_tsm_: i_thread_state)
+  : Lemma (requires (related_addm_param a i_a /\ addm_precond a /\
+                     addm_postcond a tsm_ /\
+                     IV.addm_postcond i_a i_tsm_))
+          (ensures (related_tsm tsm_ i_tsm_))
