steel/Zeta.Steel.AppSim.fsti
@@ -1,0 +1,66 @@
+module Zeta.Steel.AppSim
+
+open Zeta.Steel.ThreadStateModel
+open Zeta.Steel.Rel
+open Zeta.Steel.LogRel
+open Zeta.Steel.StoreRel
+open Zeta.Steel.ThreadRelDef
+
+module A = Zeta.App
+module AS = Zeta.AppSimulate
+module AT = Zeta.Steel.ApplicationTypes
+module GV = Zeta.GenericVerifier
+module IV = Zeta.Intermediate.Verifier
+module T = Zeta.Steel.FormatsManual
+
+val runapp_simulation (tsm: s_thread_state) (i_tsm: i_thread_state) (se: s_log_entry) (ie: i_log_entry)
+  : Lemma (requires (related_tsm tsm i_tsm /\
+                     related_log_entry se ie /\
+                     T.RunApp? se /\ not tsm.failed))
+          (ensures (let T.RunApp p = se in
+                    let tsm_ = runapp tsm p in
+                    let i_tsm_ = GV.verify_step ie i_tsm in
+                    (not tsm_.failed) ==> related_tsm tsm_ i_tsm_))
+
+let runapp_out_t
+  = let open AT in
+    fid:A.appfn_id app &
+    app_args fid &
+    app_records fid &
+    app_result fid
+
+let valid_runapp_param (tsm: s_thread_state) (se: s_log_entry)
+  = let open T in
+    RunApp? se /\
+    (let RunApp p = se in
+     let tsm_ = runapp tsm p in
+     not tsm_.failed)
+
+val runapp_output (tsm: s_thread_state)
+                  (se: s_log_entry {valid_runapp_param tsm se})
+  : GTot (o:runapp_out_t {let T.RunApp p = se in
+                          let tsm_ = runapp tsm p in
+                          tsm_.app_results = Seq.snoc tsm.app_results o})
+
+let related_output (so: runapp_out_t) (io: AS.appfn_call_res app)
+  = let (| fid, arg, inp, res  |) = so in
+    let open AS in
+    fid = io.fid_cr /\
+    arg = io.arg_cr /\
+    inp = io.inp_cr /\
+    res = io.res_cr
+
+val runapp_output_related (tsm: s_thread_state)
+                          (i_tsm: i_thread_state)
+                          (se: s_log_entry)
+                          (ie: i_log_entry)
+  : Lemma (requires (related_tsm tsm i_tsm /\
+                     related_log_entry se ie /\
+                     not tsm.failed /\
+                     valid_runapp_param tsm se))
+          (ensures (let res = runapp_output tsm se in
+                    let i_tsm_ = GV.verify_step ie i_tsm in
+                    GV.is_appfn ie /\
+                    i_tsm_.IV.valid /\
+                    (let i_res = GV.appfn_result ie i_tsm in
+                     related_output res i_res)))
