steel/Zeta.Steel.BitUtils.fst
@@ -1,0 +1,26 @@
+module Zeta.Steel.BitUtils
+
+module T = Zeta.Steel.FormatsManual
+module L = FStar.List.Tot
+module U64 = FStar.UInt64
+module BV = FStar.BV
+
+[@@"opaque_to_smt"]
+let bv_of_u256 (i:T.u256) : BV.bv_t 256 =
+  let open T in
+  let open L in
+  let bv0 = BV.bv2list (BV.int2bv #64 (U64.v (i.v0))) in
+  let bv1 = BV.bv2list (BV.int2bv #64 (U64.v (i.v1))) in
+  let bv2 = BV.bv2list (BV.int2bv #64 (U64.v (i.v2))) in
+  let bv3 = BV.bv2list (BV.int2bv #64 (U64.v (i.v3))) in
+  BV.list2bv (bv0@bv1@bv2@bv3)
+
+[@@"opaque_to_smt"]
+let bitvec_of_u256 (i:T.u256) : FStar.BitVector.bv_t 256 =
+  Seq.seq_of_list (BV.bv2list (bv_of_u256 i))
+
+let bitvec_of_u256_inj (i j:_)
+  : Lemma
+    (ensures bitvec_of_u256 i == bitvec_of_u256 j ==>
+             i == j)
+  = admit()
