steel/Zeta.Steel.GlobalRel.fst
@@ -1,0 +1,179 @@
+module Zeta.Steel.GlobalRel
+
+open FStar.Classical
+open Zeta.MultiSet.SSeq
+module GT = Zeta.Generic.Thread
+module TSM = Zeta.Steel.ThreadStateModel
+module HA = Zeta.Steel.HashAccumulator
+module MS = Zeta.MultiSet
+module ThreadRel = Zeta.Steel.ThreadRel
+
+let to_ilog_idx (logs: verifiable_logs) (i: nat{i < n_threads_v})
+  : GTot (l:i_log {GT.verifiable (i,l)})
+  = let t = U16.uint_to_t i in
+    let tl = index logs t in
+    let tsm = to_tsm tl in
+    let (_,l) = to_ilog tsm in
+    l
+
+let to_ilog (logs: verifiable_logs)
+  : GTot (i_logs: i_verifiable_logs {Seq.length i_logs = n_threads_v})
+  = Seq.init_ghost n_threads_v (fun i -> to_ilog_idx logs i)
+
+let all_app_fcrs_rel (ep: epoch_id) (logs: verifiable_logs)
+  : Lemma (ensures (let s_fcrs = all_app_fcrs ep logs in
+                    let i_logs = to_ilog logs in
+                    let i_ep = lift_epoch ep in
+                    let i_fcrs = GG.app_fcrs_within_ep i_ep i_logs in
+                    s_fcrs = i_fcrs))
+  = let s_fcrs = all_app_fcrs ep logs in
+    let i_logs = to_ilog logs in
+    let i_ep = lift_epoch ep in
+    let i_fcrs = GG.app_fcrs_within_ep i_ep i_logs in
+
+    let aux (i:_)
+      : Lemma (ensures (Seq.index s_fcrs i == Seq.index i_fcrs i))
+      = let t = U16.uint_to_t i in
+        let tl = index logs t in
+        assert(app_fcrs ep tl == Seq.index s_fcrs i);
+        spec_rel_implies_same_fcrs ep tl;
+        ()
+    in
+    forall_intro aux;
+    assert(Seq.equal s_fcrs i_fcrs);
+    ()
+
+let aggregate_add_hash (logs: all_logs) (ep: epoch_id)
+  : GTot hash_value_t
+  = let tsms = TSM.run_all _ logs in
+    let aeh = TSM.aggregate_epoch_hashes tsms ep in
+    aeh.hadd
+
+let aggregate_evict_hash (logs: all_logs) (ep: epoch_id)
+  : GTot hash_value_t
+  = let tsms = TSM.run_all _ logs in
+    let aeh = TSM.aggregate_epoch_hashes tsms ep in
+    aeh.hevict
+
+let certified_epoch_aggregate_hashes_equal (logs: all_logs) (ep: epoch_id {epoch_is_certified logs ep})
+  : Lemma (ensures (aggregate_add_hash logs ep = aggregate_evict_hash logs ep))
+  = ()
+
+let all_valid_tsms = tsms: Seq.seq thread_state_model
+    {forall i. ThreadRel.valid (Seq.index tsms i)}
+
+let all_epoch_completed (ep: epoch_id) (tsms: Seq.seq thread_state_model)
+  = forall i. let tsm = Seq.index tsms i in
+          let hash = Map.sel tsm.epoch_hashes ep in
+          hash.epoch_complete
+
+let all_add_sets  (tsms: all_valid_tsms) (ep: epoch_id)
+  : GTot (Seq.seq mset)
+  = let i_ep = lift_epoch ep in
+    Seq.init_ghost (Seq.length tsms) (fun i -> add_set (Seq.index tsms i) i_ep)
+
+let all_add_sets_cons (tsms: all_valid_tsms {Seq.length tsms > 0}) (ep: epoch_id)
+  : Lemma (ensures (let add_sets = all_add_sets tsms ep in
+                    let i_ep = lift_epoch ep in
+                    Seq.tail add_sets == all_add_sets (Seq.tail tsms) ep /\
+                    Seq.head add_sets == add_set (Seq.head tsms) i_ep))
+  = let add_sets = all_add_sets tsms ep in
+    let i_ep = lift_epoch ep in
+    assert (Seq.head add_sets == add_set (Seq.head tsms) i_ep);
+    let tail = Seq.tail tsms in
+
+    let tail_add_sets = Seq.tail add_sets in
+    let add_sets_tail = all_add_sets tail ep in
+
+    let aux (i:_)
+      : Lemma (ensures (Seq.index add_sets_tail i == Seq.index tail_add_sets i))
+      = ()
+    in
+    forall_intro aux;
+    assert(Seq.equal add_sets_tail tail_add_sets);
+    ()
+
+let union_all_add_set (tsms: all_valid_tsms) (ep: epoch_id)
+  : GTot mset
+  =  union_all (all_add_sets tsms ep)
+
+let lemma_all_add_set_cons (tsms: all_valid_tsms {Seq.length tsms > 0}) (ep: epoch_id)
+  : Lemma (ensures (let tail = Seq.tail tsms in
+                    let hd = Seq.head tsms in
+                    let i_ep = lift_epoch ep in
+                    union_all_add_set tsms ep ==
+                    MS.union (add_set hd i_ep)
+                             (union_all_add_set tail ep)))
+  = all_add_sets_cons tsms ep;
+    union_all_cons (all_add_sets tsms ep)
+
+let union_all_evict_set (tsms: all_valid_tsms) (ep: epoch_id)
+  : GTot mset
+  = let i_ep= lift_epoch ep in
+    let sms = Seq.init_ghost (Seq.length tsms) (fun i -> evict_set (Seq.index tsms i) i_ep) in
+    union_all sms
+
+let rec aggregate_epoch_hashes_prop (eid: epoch_id) (tsms: all_valid_tsms {all_epoch_completed eid tsms})
+  : Lemma (ensures (let aeh = TSM.aggregate_epoch_hashes tsms eid in
+                    aeh.hadd = ms_hashfn (union_all_add_set tsms eid)))
+          (decreases (Seq.length tsms))
+  = let add_set_union = union_all_add_set tsms eid in
+    let i_ep = lift_epoch eid in
+    let aeh = TSM.aggregate_epoch_hashes tsms eid in
+
+    if Seq.length tsms = 0 then (
+      union_all_empty (all_add_sets tsms eid);
+      lemma_hashfn_empty()
+    )
+    else (
+      let tsms' = Seq.tail tsms in
+      assert (forall i. ThreadRel.valid (Seq.index tsms' i));
+      assert(all_epoch_completed eid tsms');
+      aggregate_epoch_hashes_prop eid tsms';
+      let hd = Seq.head tsms in
+      assert(not hd.failed);
+      let tl_hash = aggregate_epoch_hashes tsms' eid in
+      assert(tl_hash.hadd = ms_hashfn (union_all_add_set tsms' eid));
+      let hd_hash = Map.sel hd.epoch_hashes eid in
+      assert(hd_hash.epoch_complete);
+      assert(aeh.hadd = HA.aggregate_hashes hd_hash.hadd tl_hash.hadd);
+      valid_hadd_prop eid hd;
+      assert(hd_hash.hadd = ms_hashfn (add_set hd i_ep));
+      lemma_all_add_set_cons tsms eid;
+      lemma_union (add_set hd i_ep) (union_all_add_set tsms' eid);
+      ()
+    )
+
+let to_tsms (logs: verifiable_logs)
+  : all_valid_tsms
+  = //let tsms = Seq.init (Seq.length logs) (fun i -> to_tsm (index logs i)) in
+    admit()
+
+
+#push-options "--fuel 1 --ifuel 1 --query_stats"
+
+let aggr_add_hash_correct (logs: verifiable_logs) (ep: epoch_id)
+  : Lemma (requires (epoch_is_certified logs ep))
+          (ensures (let gl = to_ilog logs in
+                    let i_ep = lift_epoch ep in
+                    let add_set = GG.add_set i_ep gl in
+                    let h = aggregate_add_hash logs ep in
+                    h = ms_hashfn add_set))
+  = let h = aggregate_add_hash logs ep in
+    let tsms = run_all _ logs in
+    //assert (forall i. ThreadRel.valid (Seq.index tsms i));
+
+
+
+  admit()
+
+#pop-options
+
+let aggr_evict_hash_correct (logs: verifiable_logs) (ep: epoch_id)
+  : Lemma (requires (epoch_is_certified logs ep))
+          (ensures (let gl = to_ilog logs in
+                    let i_ep = lift_epoch ep in
+                    let evict_set = GG.evict_set i_ep gl in
+                    let h = aggregate_evict_hash logs ep in
+                    h = ms_hashfn evict_set))
+  = admit()
