steel/Zeta.Steel.LogRel.fst
@@ -1,0 +1,30 @@
+module Zeta.Steel.LogRel
+
+let lift_log_entry (se: s_log_entry {valid_log_entry se})
+  : ie: i_log_entry { related_log_entry se ie }
+  = admit()
+
+let lift_log (sl: s_log {valid_log sl})
+  : il:i_log {related_log sl il}
+  = admit()
+
+let lift_log_snoc (sl: s_log {valid_log sl}) (se: s_log_entry {valid_log_entry se})
+  : Lemma (requires (let sl_ = Seq.snoc sl se in
+                     valid_log sl_))
+          (ensures (let il = lift_log sl in
+                    let ie = lift_log_entry se in
+                    let sl_ = Seq.snoc sl se in
+                    let il_ = lift_log sl_ in
+                    let i = Seq.length sl in
+                    il_ == Seq.snoc il ie /\
+                    Seq.index il_ i = ie))
+  = admit()
+
+let prefix_of_valid_valid (l: s_log {valid_log l}) (i: nat{ i <= Seq.length l})
+  : Lemma (ensures (let l' = SA.prefix l i in
+                    valid_log l'))
+  = admit()
+
+let lift_prefix_commute (l: s_log {valid_log l}) (i: nat{ i <= Seq.length l})
+  : Lemma (ensures (lift_log (SA.prefix l i) == SA.prefix (lift_log l) i))
+  = admit()
