steel/Zeta.Steel.StoreRel.fst
@@ -1,0 +1,310 @@
+module Zeta.Steel.StoreRel
+
+open FStar.Classical
+
+module IS = Zeta.Intermediate.Store
+module TSM = Zeta.Steel.ThreadStateModel
+
+let lift_store (ss: s_store)
+  : is: i_store { related_store ss is }
+  = admit()
+
+#push-options "--fuel 1 --ifuel 1 --query_stats"
+
+let lemma_related_implies_parent_props (st: s_store) (i_st: i_store)
+  : Lemma (requires (related_store st i_st))
+          (ensures (parent_props st))
+  = let aux (s:_)
+      : Lemma (ensures (parent_props_local st s))
+      = let i_s = U16.v s in
+        eliminate forall i. related_store_entry_opt (Seq.index st i) (Seq.index i_st i)
+        with i_s;
+        eliminate forall i. IS.parent_props_local i_st i
+        with i_s;
+        ()
+    in
+    forall_intro aux
+
+let lemma_related_implies_points_to_inuse (st: s_store) (i_st: i_store)
+  : Lemma (requires (related_store st i_st))
+          (ensures (points_to_inuse st))
+  = let aux (s1 s2:_)
+      : Lemma (ensures (points_to_inuse_local st s1 s2))
+      = let i_s1 = U16.v s1 in
+        let i_s2 = U16.v s2 in
+        eliminate forall i. related_store_entry_opt (Seq.index st i) (Seq.index i_st i)
+        with i_s1;
+        eliminate forall i. related_store_entry_opt (Seq.index st i) (Seq.index i_st i)
+        with i_s2;
+        eliminate forall i1 i2. IS.points_to_inuse_local i_st i_s1 i_s2
+        with i_s1 i_s2;
+        ()
+    in
+    forall_intro_2 aux
+
+let lemma_related_implies_no_self_edges (st: s_store) (i_st: i_store)
+  : Lemma (requires (related_store st i_st))
+          (ensures (no_self_edges st))
+  = let aux (s:_)
+      : Lemma (ensures (no_self_edges_local st s))
+      = let i_s = U16.v s in
+        eliminate forall i. related_store_entry_opt (Seq.index st i) (Seq.index i_st i)
+        with i_s;
+        eliminate forall i. IS.no_self_edge_local i_st i
+        with i_s;
+        ()
+    in
+    forall_intro aux
+
+#pop-options
+
+let lemma_related_implies_all_props (st: s_store) (i_st: i_store)
+  : Lemma (requires (related_store st i_st))
+          (ensures (all_props st))
+  = lemma_related_implies_parent_props st i_st;
+    lemma_related_implies_points_to_inuse st i_st;
+    lemma_related_implies_no_self_edges st i_st
+
+let lemma_update_value (tsm: TSM.thread_state_model)
+                       (s: T.slot {TSM.has_slot tsm s})
+                       (v: T.value {TSM.is_value_of (TSM.key_of_slot tsm s) v})
+  : Lemma (ensures (let tsm_ = TSM.update_value tsm s v in
+                    identical_except_store tsm tsm_ /\
+                    identical_except tsm.store tsm_.store s /\
+                    inuse_slot tsm_.store s /\
+                    (let Some e = get_slot tsm.store s in
+                     let Some e_ = get_slot tsm_.store s in
+                     e.key = e_.key /\ e_.value = v /\ e.add_method = e_.add_method /\
+                     e.l_child_in_store = e_.l_child_in_store /\
+                     e.r_child_in_store = e_.r_child_in_store)))
+  = let tsm_ = TSM.update_value tsm s v in
+
+    assert (identical_except_store tsm tsm_);
+    assert (inuse_slot tsm_.store s);
+    let aux (s':_)
+      : Lemma (ensures (s' <> s ==> get_slot tsm.store s' == get_slot tsm_.store s'))
+      = if s' <> s then ()
+    in
+    forall_intro aux;
+    assert (identical_except tsm.store tsm_.store s);
+    ()
+
+let lemma_madd_to_store (tsm: TSM.thread_state_model)
+                        (s: T.slot)
+                        (k: T.key)
+                        (v: T.value)
+                        (s':T .slot)
+                        (d: bool)
+  : Lemma (requires (madd_to_store_reqs tsm s k v s' d))
+          (ensures (let tsm_ = TSM.madd_to_store tsm s k v s' d in
+                    let od = not d in
+                    let open TSM in
+                    identical_except_store tsm tsm_ /\
+                    identical_except2 tsm.store tsm_.store s s' /\
+
+                    // nothing changes in slot s' except it now points to s in direction d
+                    inuse_slot tsm_.store s' /\
+                    stored_key tsm_.store s' = stored_key tsm.store s' /\
+                    stored_value tsm_.store s' = stored_value tsm.store s' /\
+                    add_method_of tsm_.store s' = add_method_of tsm.store s' /\
+                    points_to_dir tsm_.store s' d s /\
+                    points_to_info tsm_.store s' od = points_to_info tsm.store s' od /\
+
+                    // slot s contains (k, v, MAdd) and points to nothing
+                    inuse_slot tsm_.store s /\
+                    (let Some e = get_slot tsm_.store s in
+                     e.key = k /\ e.value = v /\ e.add_method = MAdd /\
+                     e.l_child_in_store = None /\ e.r_child_in_store = None /\
+                     e.parent_slot = Some (s', d))))
+  = let open TSM in
+    let tsm_ = madd_to_store tsm s k v s' d in
+
+    assert (identical_except_store tsm tsm_);
+    let aux (s':_)
+      : Lemma (ensures (s' <> s ==> s' <> s' ==> get_slot tsm.store s' == get_slot tsm_.store s'))
+      = ()
+    in
+    forall_intro aux;
+    ()
+
+let lemma_madd_to_store_split (tsm: TSM.thread_state_model)
+                              (s: T.slot)
+                              (k: T.key)
+                              (v: T.value)
+                              (s':T.slot)
+                              (d d2:bool)
+  : Lemma (requires (madd_to_store_split_reqs tsm s k v s' d d2 /\ all_props tsm.store))
+          (ensures (let tsm_ = TSM.madd_to_store_split tsm s k v s' d d2 in
+                    let od = not d in
+                    let od2 = not d2 in
+                    let s2 = pointed_slot tsm.store s' d in
+                    let open TSM in
+
+                    identical_except_store tsm tsm_ /\
+                    identical_except3 tsm.store tsm_.store s s' s2 /\
+
+                    // nothing changes in slot s', except it now points to s in direction d
+                    inuse_slot tsm_.store s' /\
+                    stored_key tsm_.store s' = stored_key tsm.store s' /\
+                    stored_value tsm_.store s' = stored_value tsm.store s' /\
+                    add_method_of tsm_.store s' = add_method_of tsm.store s' /\
+                    points_to_dir tsm_.store s' d s /\
+                    points_to_info tsm_.store s' od = points_to_info tsm.store s' od /\
+
+                    // slot s contains (k, v, MAdd) and points to s2 along direction d2
+                    inuse_slot tsm_.store s /\
+                    stored_key tsm_.store s = k /\ stored_value tsm_.store s = v /\
+                    add_method_of tsm_.store s = MAdd /\
+                    points_to_none tsm_.store s od2 /\
+                    points_to_dir tsm_.store s d2 s2 /\
+                    has_parent tsm_.store s /\
+                    parent_slot tsm_.store s = s' /\
+                    parent_dir tsm_.store s = d /\
+
+                    inuse_slot tsm_.store s2 /\ inuse_slot tsm.store s2 /\
+                    has_parent tsm_.store s2 /\
+                    parent_slot tsm_.store s2 = s /\
+                    parent_dir tsm_.store s2 = d2 /\
+
+                    (let Some e = get_slot tsm.store s2 in
+                     let Some e_ = get_slot tsm_.store s2 in
+                     e.key = e_.key /\ e.value = e_.value /\
+                     e.add_method = e_.add_method /\
+                     e.l_child_in_store = e_.l_child_in_store /\
+                     e.r_child_in_store = e_.r_child_in_store)))
+  = let tsm_ = TSM.madd_to_store_split tsm s k v s' d d2 in
+    let od = not d in
+    let od2 = not d2 in
+    let s2 = pointed_slot tsm.store s' d in
+    let open TSM in
+
+    assert (identical_except_store tsm tsm_);
+    assume (identical_except3 tsm.store tsm_.store s s' s2);
+
+    assert (points_to_dir tsm.store s' d s2);
+    eliminate forall (s1 s2: T.slot). points_to_inuse_local tsm.store s1 s2
+    with s' s2;
+
+    assert(inuse_slot tsm_.store s' /\
+                    stored_key tsm_.store s' = stored_key tsm.store s' /\
+                    stored_value tsm_.store s' = stored_value tsm.store s' /\
+                    add_method_of tsm_.store s' = add_method_of tsm.store s' /\
+                    points_to_dir tsm_.store s' d s /\
+                    points_to_info tsm_.store s' od = points_to_info tsm.store s' od);
+    assert(inuse_slot tsm_.store s /\
+                    stored_key tsm_.store s = k /\ stored_value tsm_.store s = v /\
+                    add_method_of tsm_.store s = MAdd /\
+                    points_to_none tsm_.store s od2 /\
+                    points_to_dir tsm_.store s d2 s2 /\
+                    has_parent tsm_.store s /\
+                    parent_slot tsm_.store s = s' /\
+                    parent_dir tsm_.store s = d);
+    assert(inuse_slot tsm_.store s2 /\ inuse_slot tsm.store s2);
+    assert(has_parent tsm_.store s2);
+    assert(parent_slot tsm_.store s2 = s);
+    assert(parent_dir tsm_.store s2 = d2);
+    assert (s <> s');
+    assert (s <> s2);
+    assert (s' <> s2);
+    let st = tsm.store in
+    match get_entry tsm s' with
+    | Some r' ->
+      let p = (s', d) in
+      let s2_opt = child_slot r' d in
+      assert (s2_opt = Some s2);
+      //match s2_opt with
+      //| None -> assert(False); ()
+      //| Some s2 ->
+        //if U16.v s2 >= Seq.length st
+        //then
+        //begin
+          //assert(False); ()
+        //end
+        //else //match Seq.index st (U16.v s2) with
+        //| None -> assert(False); ()
+        //| Some r2 ->
+                 //let e = mk_entry_full k v MAdd None None (Some p) in
+                 //let e = update_child e d2 s2 in
+                 //let e' = update_child r' d s in
+                 //let p2new = s, d2 in
+                 //let e2 = update_parent_slot r2 p2new in
+          //assert(Some e2 == get_slot tsm_.store s2);
+          //assert(Some r2 == get_slot tsm.store s2);
+          //assert(e2.value = r2.value);
+
+
+    (*
+    assert(let Some e = get_slot tsm.store s2 in
+           let Some e_ = get_slot tsm_.store s2 in
+            e == r2 /\ e_ == e2 /\
+           e.key = e_.key /\ e.add_method = e_.add_method /\
+                     e.key = e_.key /\ e.value = e_.value /\
+                     e.add_method = e_.add_method /\
+                     e.l_child_in_store = e_.l_child_in_store /\
+                     e.r_child_in_store = e_.r_child_in_store);
+                    *)
+    ()
+
+let lemma_mevict_from_store (tsm: s_thread_state)
+                            (s: T.slot)
+                            (s': T.slot)
+                            (d: bool)
+  : Lemma (requires (s <> s' /\ TSM.has_slot tsm s'))
+          (ensures (let od = not d in
+                    let st = tsm.store in
+                    let open TSM in
+                    let tsm_ = mevict_from_store tsm s s' d in
+                    let st_ = tsm_.store in
+
+                    // st and st_ are identical except at s, s'
+                    identical_except2 st st_ s s' /\
+
+                    // slot s is empty after update
+                    empty_slot st_ s /\
+
+                    // nothing changes in slot s', except it points to none in direction d
+                    inuse_slot st_ s' /\
+                    stored_key st_ s' = stored_key st s' /\
+                    stored_value st_ s' = stored_value st s' /\
+                    add_method_of st_ s' = add_method_of st s' /\
+                    points_to_info st_ s' od = points_to_info st s' od /\
+                    points_to_none st_ s' d /\
+                    parent_info st_ s' = parent_info st s'))
+  = let od = not d in
+    let st = tsm.store in
+    let open TSM in
+    let tsm_ = mevict_from_store tsm s s' d in
+    let st_ = tsm_.store in
+
+    let aux (si:_)
+      : Lemma (ensures (si <> s ==> si <> s' ==> get_slot st si == get_slot st_ si))
+      = if si <> s && si <> s' then
+           ()
+    in
+    forall_intro aux;
+    assert (identical_except2 st st_ s s');
+
+    assert (empty_slot st_ s);
+    ()
+
+let lemma_bevict_from_store (tsm: s_thread_state)
+                            (s: T.slot)
+  : Lemma (ensures (let st = tsm.store in
+                    let open TSM in
+                    let tsm_ = bevict_from_store tsm s in
+                    let st_ = tsm_.store in
+                    identical_except st st_ s /\
+                    empty_slot st_ s))
+  = let open TSM in
+    let st = tsm.store in
+    let tsm_ = bevict_from_store tsm s in
+    let st_ = tsm_.store in
+
+    let aux (s':_)
+      : Lemma (ensures (s' <> s ==> get_slot st s' == get_slot st_ s'))
+      = if s' <> s then ()
+    in
+    forall_intro aux;
+    assert (identical_except st st_ s);
+
+    ()
