steel/Zeta.Steel.ThreadRel.fst
@@ -1,0 +1,1616 @@
+module Zeta.Steel.ThreadRel
+
+open FStar.Classical
+open Zeta.Steel.ThreadSim
+open Zeta.Steel.AppSim
+
+module A = Zeta.App
+module M = Zeta.Merkle
+module R = Zeta.Record
+module T = Zeta.Steel.FormatsManual
+module S = FStar.Seq
+module SA = Zeta.SeqAux
+module KU = Zeta.Steel.KeyUtils
+module GK = Zeta.GenKey
+module IS = Zeta.Intermediate.Store
+module SS = Zeta.Steel.StoreRel
+module HA = Zeta.Steel.HashAccumulator
+
+#push-options "--fuel 1 --ifuel 2 --query_stats"
+
+let addm_processed_entries_props (tsm: thread_state_model) (e: s_log_entry {T.AddM? e})
+  : Lemma (ensures (let open T in
+                    let AddM p = e in
+                    let tsm_ = vaddm tsm p.s p.s' (Inl (p.k, p.v)) in
+                    tsm_.processed_entries == tsm.processed_entries))
+  = ()
+
+let addm_thread_id_prop (tsm: thread_state_model) (e: s_log_entry {T.AddM? e})
+  : Lemma (ensures (let open T in
+                    let AddM p = e in
+                    let tsm_ = vaddm tsm p.s p.s' (Inl (p.k, p.v)) in
+                    tsm_.thread_id == tsm.thread_id))
+  = ()
+
+let addm_valid_log_entry_prop (tsm: thread_state_model) (e: s_log_entry {T.AddM? e})
+  : Lemma (ensures (let open T in
+                    let AddM p = e in
+                    let tsm_ = vaddm tsm p.s p.s' (Inl (p.k, p.v)) in
+                    not tsm_.failed ==> valid_log_entry e))
+  = ()
+
+let addmapp_processed_entries_props (tsm: thread_state_model) (e: s_log_entry {T.AddMApp? e})
+  : Lemma (ensures (let open T in
+                    let AddMApp p = e in
+                    let tsm_ = vaddm tsm p.s p.s' (Inr p.rest) in
+                    tsm_.processed_entries == tsm.processed_entries))
+  = ()
+
+
+let addmapp_thread_id_prop (tsm: thread_state_model) (e: s_log_entry {T.AddMApp? e})
+  : Lemma (ensures (let open T in
+                    let AddMApp p = e in
+                    let tsm_ = vaddm tsm p.s p.s' (Inr p.rest) in
+                    tsm_.thread_id == tsm.thread_id))
+  = ()
+
+let addmapp_valid_log_entry_prop (tsm: thread_state_model) (e: s_log_entry {T.AddMApp? e})
+  : Lemma (ensures (let open T in
+                    let AddMApp p = e in
+                    let tsm_ = vaddm tsm p.s p.s' (Inr p.rest) in
+                    not tsm_.failed ==> valid_log_entry e))
+  = ()
+
+#pop-options
+
+let runapp_slots_prop (tsm: thread_state_model) (slots: S.seq T.slot_id)
+  = forall (s:U16.t). Seq.contains slots s ==>
+                  has_slot tsm s /\
+                  T.ApplicationKey? (key_of_slot tsm s)
+
+let rec read_slots_valid_prop (tsm: thread_state_model) (slots: S.seq T.slot_id)
+  : Lemma (ensures (let or = read_slots tsm slots in
+                    Some? or ==> (forall i. valid_slot (S.index slots i))))
+          (decreases (S.length slots))
+  = let or = read_slots tsm slots in
+    if Some? or && S.length slots > 0 then (
+      let hd = S.head slots in
+      let tl = S.tail slots in
+      Classical.forall_intro (Seq.contains_cons hd tl);
+
+      read_slots_valid_prop tsm tl;
+      assert(valid_slot hd);
+      let aux (i:_)
+        : Lemma (ensures (valid_slot (S.index slots i)))
+        = if i > 0 then
+            assert(valid_slot (S.index tl (i-1)))
+      in
+      forall_intro aux
+    )
+
+let rec write_slots_non_store_prop
+  (tsm: thread_state_model)
+  (slots: _ {runapp_slots_prop tsm slots})
+  (values: S.seq (app_value_nullable app.adm) {S.length slots == S.length values})
+  : Lemma (ensures (let tsm_ = write_slots tsm slots values in
+                    tsm_.failed == tsm.failed /\
+                    tsm_.clock == tsm.clock /\
+                    tsm_.epoch_hashes == tsm.epoch_hashes /\
+                    tsm_.thread_id == tsm.thread_id /\
+                    tsm_.processed_entries == tsm.processed_entries /\
+                    tsm_.app_results == tsm.app_results))
+          (decreases (S.length slots))
+  = let tsm_ = write_slots tsm slots values in
+    if S.length slots > 0 then (
+      let hd_slot = S.head slots in
+      let tl = S.tail slots in
+      assert(slots `S.equal` S.cons hd_slot tl);
+      Classical.forall_intro (Seq.contains_cons hd_slot tl);
+      let hd_value =
+        match Seq.head values with
+        | Null -> T.DValue None
+        | DValue d -> T.DValue (Some d)
+      in
+      let tsm = update_value tsm hd_slot hd_value in
+      write_slots_non_store_prop tsm (S.tail slots) (S.tail values)
+    )
+
+(* do all the runapp_checks satisfy *)
+let runapp_checks_sat (tsm: thread_state_model) (pl: T.runApp_payload)
+  : GTot bool
+  = let open T in
+    if not (Map.contains app.tbl pl.fid)
+    then false //unknown fid
+    else (
+      match AT.spec_app_parser pl.fid pl.rest.ebytes with
+      | None -> false //parsing failed
+      | Some ((arg, slots), len) ->
+        if len <> U32.v pl.rest.len
+        then false //parsing failed, some bytes not consumed
+        else if not (Zeta.SeqAux.distinct_elems_comp slots)
+        then false //not distinct slots
+        else
+          let fsig = Map.sel app.tbl pl.fid in
+          match read_slots tsm slots with
+          | None -> false
+          | Some recs ->
+            if not (check_distinct_keys recs)
+            then false
+            else (
+              let res = fsig.f arg recs in
+              match res with
+              | ( Fn_failure, _, _) -> false
+              | (_, res, out_vals) -> true
+            )
+        )
+
+let runapp_checks_unsat_prop (tsm: thread_state_model) (pl: T.runApp_payload)
+  : Lemma (ensures (not (runapp_checks_sat tsm pl) ==> fail tsm == runapp tsm pl))
+  = ()
+
+let runapp_non_store_prop (tsm: thread_state_model) (e: s_log_entry {T.RunApp? e})
+  : Lemma (ensures (let open T in
+                    let RunApp p = e in
+                    let tsm_ = runapp tsm p in
+                    tsm_.processed_entries == tsm.processed_entries /\
+                    tsm_.thread_id = tsm.thread_id))
+  = let open T in
+    let RunApp p = e in
+    let tsm_ = runapp tsm p in
+    runapp_checks_unsat_prop tsm p;
+    if runapp_checks_sat tsm p then
+      match AT.spec_app_parser p.fid p.rest.ebytes with
+      | Some ((arg, slots), len) ->
+        let fsig = Map.sel app.tbl p.fid in
+        match read_slots tsm slots with
+        | Some recs ->
+          let res = fsig.f arg recs in
+          match res with
+          | _, res, out_vals ->
+            let tsm = {tsm with app_results=Seq.Properties.snoc tsm.app_results (| p.fid, arg, recs, res |)} in
+            write_slots_non_store_prop tsm slots out_vals
+
+let runapp_valid_log_entry_prop (tsm: thread_state_model) (e: s_log_entry {T.RunApp? e})
+  : Lemma (ensures (let open T in
+                    let RunApp p = e in
+                    let tsm_ = runapp tsm p in
+                    not tsm_.failed ==> valid_log_entry e))
+  = let open T in
+    let RunApp p = e in
+    let tsm_ = runapp tsm p in
+    runapp_checks_unsat_prop tsm p;
+    if runapp_checks_sat tsm p && not tsm_.failed then
+      match AT.spec_app_parser p.fid p.rest.ebytes with
+      | Some ((arg, slots), len) ->
+        read_slots_valid_prop tsm slots
+
+let verify_step_model_processed_entries_prop (tsm: thread_state_model) (e: s_log_entry)
+  : Lemma (ensures (let tsm_ = verify_step_model tsm e in
+                    not tsm.failed ==> tsm_.processed_entries == Seq.snoc tsm.processed_entries e))
+          [SMTPat (verify_step_model tsm e)]
+  = let open T in
+    if not tsm.failed then
+      match e with
+      | AddM _ -> addm_processed_entries_props tsm e
+      | AddMApp _ -> addmapp_processed_entries_props tsm e
+      | RunApp _ -> runapp_non_store_prop tsm e
+      | _ -> ()
+
+let verify_step_model_thread_id_prop (tsm: thread_state_model) (e: s_log_entry)
+  : Lemma (ensures (let tsm_ = verify_step_model tsm e in
+                    tsm_.thread_id = tsm.thread_id))
+          [SMTPat (verify_step_model tsm e)]
+  = let open T in
+    match e with
+    | AddM _ -> addm_thread_id_prop tsm e
+    | AddMApp _ -> addmapp_thread_id_prop tsm e
+    | RunApp _ -> runapp_non_store_prop tsm e
+    | _ -> ()
+
+let verify_step_model_valid_log_entry_prop (tsm: thread_state_model) (e: s_log_entry)
+  : Lemma (ensures (let tsm_ = verify_step_model tsm e in
+                    not tsm_.failed ==> valid_log_entry e))
+          [SMTPat (verify_step_model tsm e)]
+  = let open T in
+    let tsm_ = verify_step_model tsm e in
+    if not tsm_.failed then (
+      match e with
+      | AddM _ -> addm_valid_log_entry_prop tsm e
+      | AddMApp _ -> addmapp_valid_log_entry_prop tsm e
+      | RunApp _ -> runapp_valid_log_entry_prop tsm e
+      | _ -> ()
+    )
+
+let rec run_implies_processed_entries (tid: AT.tid) (l: s_log)
+  : Lemma (ensures (let tsm = run tid l in
+                    tsm.failed \/
+                    tsm.processed_entries == l))
+          (decreases (S.length l))
+  = let tsm = run tid l in
+    if S.length l = 0 then
+      S.lemma_empty l
+    else (
+      let i = S.length l - 1 in
+      let l' = SA.prefix l i in
+      let e = S.index l i in
+      run_implies_processed_entries tid l';
+      let tsm' = run tid l' in
+
+      if not tsm'.failed && not tsm.failed then (
+        verify_step_model_processed_entries_prop tsm' e;
+        SA.lemma_hprefix_append_telem l
+      )
+    )
+
+let rec run_implies_thread_id (tid: AT.tid) (l: s_log)
+  : Lemma (ensures (let tsm = run tid l in
+                    tsm.thread_id = tid))
+          (decreases (S.length l))
+  = let tsm = run tid l in
+    if S.length l > 0 then (
+      let i = S.length l - 1 in
+      let l' = SA.prefix l i in
+      let e = S.index l i in
+      run_implies_thread_id tid l';
+      verify_step_model_thread_id_prop (run tid l') e;
+      ()
+    )
+
+let run_implies_valid (tid: AT.tid) (l: s_log)
+  : Lemma (ensures (let tsm = run tid l in
+                    tsm.failed \/ valid tsm))
+  = let tsm = run tid l in
+    run_implies_processed_entries tid l;
+    run_implies_thread_id tid l
+
+let rec run_implies_valid_log (tid: AT.tid) (l: s_log)
+  : Lemma (ensures (let tsm = run tid l in
+                    not tsm.failed ==> valid_log l))
+          (decreases (S.length l))
+  = let tsm = run tid l in
+    if S.length l > 0 then (
+      let i = S.length l - 1 in
+      let l' = SA.prefix l i in
+      let e = S.index l i in
+      let tsm' = run tid l' in
+      run_implies_valid_log tid l';
+      verify_step_model_valid_log_entry_prop (run tid l') e;
+      if not tsm.failed then (
+        assert(valid_log l');
+        assert(valid_log_entry e);
+        let aux (j:_)
+          : Lemma (ensures (valid_log_entry (S.index l j)))
+          = if j < i then
+              eliminate forall i. valid_log_entry (S.index l' i) with j
+        in
+        forall_intro aux
+      )
+    )
+
+let valid_implies_valid_log (tsm: valid_tsm)
+  : Lemma (ensures (valid_log tsm.processed_entries))
+  = run_implies_valid tsm.thread_id tsm.processed_entries;
+    run_implies_valid_log tsm.thread_id tsm.processed_entries
+
+let verify_step_model_extends_validity (tsm: valid_tsm) (e: s_log_entry)
+  : Lemma (ensures (let tsm_ = verify_step_model tsm e in
+                    not tsm_.failed ==> valid tsm_))
+          [SMTPat (verify_step_model tsm e)]
+  = let l = tsm.processed_entries in
+    let t = tsm.thread_id in
+    let l_ = SA.append1 l e in
+    let tsm_ = run t l_ in
+    SA.lemma_prefix1_append l e;
+    assert(l == SA.prefix l_ (S.length l));
+    run_implies_valid t l_
+
+let to_i_tl (tsm: valid_tsm {spec_rel_base tsm})
+  : GTot (Zeta.Intermediate.Thread.verifiable_log i_vcfg)
+  = let i_log = lift_log tsm.processed_entries in
+    let i_tid = lift_tid tsm.thread_id in
+    i_tid, i_log
+
+let to_i_tsm (tsm: valid_tsm {spec_rel_base tsm})
+  : GTot (i_thread_state)
+  = Zeta.Generic.Thread.state (to_i_tl tsm)
+
+let verify_step_model_lifted_log_prop (tsm:_ {spec_rel_base tsm}) (e: s_log_entry)
+  : Lemma (requires (let tsm_ = verify_step_model tsm e in
+                     not tsm_.failed))
+          (ensures (let tsm_ = verify_step_model tsm e in
+                    let i_log = lift_log tsm.processed_entries in
+                    let i_e = lift_log_entry e in
+                    let i_log_ = lift_log tsm_.processed_entries in
+                    let i = Seq.length i_log in
+                    i_log_ == Seq.snoc i_log i_e /\
+                    Seq.index i_log_ i = i_e /\
+                    i_log = SA.prefix i_log_ i))
+          [SMTPat (verify_step_model tsm e)]
+  = let i_log = lift_log tsm.processed_entries in
+    let i_e = lift_log_entry e in
+    lift_log_snoc tsm.processed_entries e;
+    SA.lemma_prefix1_append i_log i_e
+
+let spec_rel_base_addm (tsm:_ {spec_rel_base tsm}) (e: s_log_entry {T.AddM? e})
+  : Lemma (ensures (let tsm_ = verify_step_model tsm e in
+                    not tsm_.failed ==> valid tsm_ /\ spec_rel_base tsm_))
+  = let open T in
+    let tid = tsm.TSM.thread_id in
+    let i_tid = lift_tid tid in
+    let tsm_ = verify_step_model tsm e in
+
+    let i_log = lift_log tsm.processed_entries in
+    let i_tsm = to_i_tsm tsm in
+
+    if not tsm_.failed then (
+      (* verify_step extends validity or fails *)
+      assert(valid tsm_);
+
+      let i_e = lift_log_entry e in
+      assert (related_log_entry e i_e);
+
+      let i_tsm_ = GV.verify_step i_e i_tsm in
+      let i_log_ = lift_log tsm_.processed_entries in
+      addm_simulation tsm i_tsm e i_e
+    )
+
+let spec_rel_base_addmapp (tsm:_ {spec_rel_base tsm}) (e: s_log_entry {T.AddMApp? e})
+  : Lemma (ensures (let tsm_ = verify_step_model tsm e in
+                    not tsm_.failed ==> valid tsm_ /\ spec_rel_base tsm_))
+  = let open T in
+    let tid = tsm.TSM.thread_id in
+    let i_tid = lift_tid tid in
+    let tsm_ = verify_step_model tsm e in
+
+    let i_log = lift_log tsm.processed_entries in
+    let i_tsm = to_i_tsm tsm in
+
+    if not tsm_.failed then (
+      (* verify_step extends validity or fails *)
+      assert(valid tsm_);
+
+      let i_e = lift_log_entry e in
+      assert (related_log_entry e i_e);
+
+      let i_tsm_ = GV.verify_step i_e i_tsm in
+      let i_log_ = lift_log tsm_.processed_entries in
+      addmapp_simulation tsm i_tsm e i_e
+    )
+
+let spec_rel_base_addb (tsm:_ {spec_rel_base tsm}) (e: s_log_entry {T.AddB? e})
+  : Lemma (ensures (let tsm_ = verify_step_model tsm e in
+                    not tsm_.failed ==> valid tsm_ /\ spec_rel_base tsm_))
+  = let open T in
+    let tid = tsm.TSM.thread_id in
+    let i_tid = lift_tid tid in
+    let tsm_ = verify_step_model tsm e in
+
+    let i_log = lift_log tsm.processed_entries in
+    let i_tsm = to_i_tsm tsm in
+
+    if not tsm_.failed then (
+      (* verify_step extends validity or fails *)
+      assert(valid tsm_);
+
+      let i_e = lift_log_entry e in
+      assert (related_log_entry e i_e);
+
+      let i_tsm_ = GV.verify_step i_e i_tsm in
+      let i_log_ = lift_log tsm_.processed_entries in
+      addb_simulation tsm i_tsm e i_e
+    )
+
+let spec_rel_base_addbapp (tsm:_ {spec_rel_base tsm}) (e: s_log_entry {T.AddBApp? e})
+  : Lemma (ensures (let tsm_ = verify_step_model tsm e in
+                    not tsm_.failed ==> valid tsm_ /\ spec_rel_base tsm_))
+  = let open T in
+    let tid = tsm.TSM.thread_id in
+    let i_tid = lift_tid tid in
+    let tsm_ = verify_step_model tsm e in
+
+    let i_log = lift_log tsm.processed_entries in
+    let i_tsm = to_i_tsm tsm in
+
+    if not tsm_.failed then (
+      (* verify_step extends validity or fails *)
+      assert(valid tsm_);
+
+      let i_e = lift_log_entry e in
+      assert (related_log_entry e i_e);
+
+      let i_tsm_ = GV.verify_step i_e i_tsm in
+      let i_log_ = lift_log tsm_.processed_entries in
+      addbapp_simulation tsm i_tsm e i_e
+    )
+
+let spec_rel_base_evictm (tsm:_ {spec_rel_base tsm}) (e: s_log_entry {T.EvictM? e})
+  : Lemma (ensures (let tsm_ = verify_step_model tsm e in
+                    not tsm_.failed ==> valid tsm_ /\ spec_rel_base tsm_))
+  = let open T in
+    let tid = tsm.TSM.thread_id in
+    let i_tid = lift_tid tid in
+    let tsm_ = verify_step_model tsm e in
+
+    let i_log = lift_log tsm.processed_entries in
+    let i_tsm = to_i_tsm tsm in
+
+    if not tsm_.failed then (
+      (* verify_step extends validity or fails *)
+      assert(valid tsm_);
+
+      let i_e = lift_log_entry e in
+      assert (related_log_entry e i_e);
+
+      let i_tsm_ = GV.verify_step i_e i_tsm in
+      let i_log_ = lift_log tsm_.processed_entries in
+      evictm_simulation tsm i_tsm e i_e
+    )
+
+let spec_rel_base_evictb (tsm:_ {spec_rel_base tsm}) (e: s_log_entry {T.EvictB? e})
+  : Lemma (ensures (let tsm_ = verify_step_model tsm e in
+                    not tsm_.failed ==> valid tsm_ /\ spec_rel_base tsm_))
+  = let open T in
+    let tid = tsm.TSM.thread_id in
+    let i_tid = lift_tid tid in
+    let tsm_ = verify_step_model tsm e in
+
+    let i_log = lift_log tsm.processed_entries in
+    let i_tsm = to_i_tsm tsm in
+
+    if not tsm_.failed then (
+      (* verify_step extends validity or fails *)
+      assert(valid tsm_);
+
+      let i_e = lift_log_entry e in
+      assert (related_log_entry e i_e);
+
+      let i_tsm_ = GV.verify_step i_e i_tsm in
+      let i_log_ = lift_log tsm_.processed_entries in
+      evictb_simulation tsm i_tsm e i_e
+    )
+
+let spec_rel_base_evictbm (tsm:_ {spec_rel_base tsm}) (e: s_log_entry {T.EvictBM? e})
+  : Lemma (ensures (let tsm_ = verify_step_model tsm e in
+                    not tsm_.failed ==> valid tsm_ /\ spec_rel_base tsm_))
+  = let open T in
+    let tid = tsm.TSM.thread_id in
+    let i_tid = lift_tid tid in
+    let tsm_ = verify_step_model tsm e in
+
+    let i_log = lift_log tsm.processed_entries in
+    let i_tsm = to_i_tsm tsm in
+
+    if not tsm_.failed then (
+      (* verify_step extends validity or fails *)
+      assert(valid tsm_);
+
+      let i_e = lift_log_entry e in
+      assert (related_log_entry e i_e);
+
+      let i_tsm_ = GV.verify_step i_e i_tsm in
+      let i_log_ = lift_log tsm_.processed_entries in
+      evictbm_simulation tsm i_tsm e i_e
+    )
+
+let spec_rel_base_nextepoch (tsm:_ {spec_rel_base tsm}) (e: s_log_entry {T.NextEpoch? e})
+  : Lemma (ensures (let tsm_ = verify_step_model tsm e in
+                    not tsm_.failed ==> valid tsm_ /\ spec_rel_base tsm_))
+  = let open T in
+    let tid = tsm.TSM.thread_id in
+    let i_tid = lift_tid tid in
+    let tsm_ = verify_step_model tsm e in
+
+    let i_log = lift_log tsm.processed_entries in
+    let i_tsm = to_i_tsm tsm in
+
+    if not tsm_.failed then (
+      (* verify_step extends validity or fails *)
+      assert(valid tsm_);
+
+      let i_e = lift_log_entry e in
+      assert (related_log_entry e i_e);
+
+      let i_tsm_ = GV.verify_step i_e i_tsm in
+      let i_log_ = lift_log tsm_.processed_entries in
+      nextepoch_simulation tsm i_tsm e i_e
+    )
+
+let spec_rel_base_verifyepoch (tsm:_ {spec_rel_base tsm}) (e: s_log_entry {T.VerifyEpoch? e})
+  : Lemma (ensures (let tsm_ = verify_step_model tsm e in
+                    not tsm_.failed ==> valid tsm_ /\ spec_rel_base tsm_))
+  = let open T in
+    let tid = tsm.TSM.thread_id in
+    let i_tid = lift_tid tid in
+    let tsm_ = verify_step_model tsm e in
+
+    let i_log = lift_log tsm.processed_entries in
+    let i_tsm = to_i_tsm tsm in
+
+    if not tsm_.failed then (
+      (* verify_step extends validity or fails *)
+      assert(valid tsm_);
+
+      let i_e = lift_log_entry e in
+      assert (related_log_entry e i_e);
+
+      let i_tsm_ = GV.verify_step i_e i_tsm in
+      let i_log_ = lift_log tsm_.processed_entries in
+      verifyepoch_simulation tsm i_tsm e i_e
+    )
+
+let spec_rel_base_runapp (tsm:_ {spec_rel_base tsm}) (e: s_log_entry {T.RunApp? e})
+  : Lemma (ensures (let tsm_ = verify_step_model tsm e in
+                    not tsm_.failed ==> valid tsm_ /\ spec_rel_base tsm_))
+  = let open T in
+    let tid = tsm.TSM.thread_id in
+    let i_tid = lift_tid tid in
+    let tsm_ = verify_step_model tsm e in
+
+    let i_log = lift_log tsm.processed_entries in
+    let i_tsm = to_i_tsm tsm in
+
+    if not tsm_.failed then (
+      (* verify_step extends validity or fails *)
+      assert(valid tsm_);
+
+      let i_e = lift_log_entry e in
+      assert (related_log_entry e i_e);
+
+      let i_tsm_ = GV.verify_step i_e i_tsm in
+      let i_log_ = lift_log tsm_.processed_entries in
+      runapp_simulation tsm i_tsm e i_e
+    )
+
+let lemma_verify_step_model_spec_rel_base (tsm:_ {spec_rel_base tsm}) (e: s_log_entry)
+  : Lemma (ensures (let tsm_ = verify_step_model tsm e in
+                    not tsm_.failed ==> valid tsm_ /\ spec_rel_base tsm_))
+          [SMTPat (verify_step_model tsm e)]
+  = let open T in
+    match e with
+    | AddM _ -> spec_rel_base_addm tsm e
+    | AddMApp _ -> spec_rel_base_addmapp tsm e
+    | AddB _ -> spec_rel_base_addb tsm e
+    | AddBApp _ -> spec_rel_base_addbapp tsm e
+    | EvictM _ -> spec_rel_base_evictm tsm e
+    | EvictB _ -> spec_rel_base_evictb tsm e
+    | EvictBM _ -> spec_rel_base_evictbm tsm e
+    | NextEpoch _ -> spec_rel_base_nextepoch tsm e
+    | VerifyEpoch _ -> spec_rel_base_verifyepoch tsm e
+    | RunApp _ -> spec_rel_base_runapp tsm e
+
+let init_tsm_valid (tid: AT.tid)
+  : Lemma (ensures (valid (init_thread_state_model tid)))
+          [SMTPat (init_thread_state_model tid)]
+  = ()
+
+let empty_store_related ()
+  : Lemma (ensures (let st = Seq.create (U16.v AT.store_size) None in
+                    let i_st = IS.empty_store i_vcfg in
+                    related_store st i_st))
+  = let st: contents = Seq.create (U16.v AT.store_size) None in
+    let i_st = IS.empty_store i_vcfg in
+
+    let aux (i:_)
+      : Lemma (ensures (related_store_entry_opt (Seq.index st i) (Seq.index i_st i)))
+      = ()
+    in
+    forall_intro aux
+
+let related_madd_to_store_root (tsm: thread_state_model)
+                               (i_st: i_store)
+                               (s: T.slot) (i_s: i_slot_id)
+                               (v: T.value) (i_v: i_val {Zeta.Record.IntV? i_v})
+  : Lemma (requires (related_store tsm.store i_st /\ related_slot s i_s /\
+                     IS.empty_slot i_st i_s /\
+                     related_val v i_v))
+          (ensures (let tsm_ = TSM.madd_to_store_root tsm s v in
+                    let st_ = tsm_.store in
+                    let i_st_ = IS.madd_to_store_root i_st i_s i_v in
+                    related_store st_ i_st_))
+  = let st = tsm.store in
+
+    eliminate forall i. related_store_entry_opt (Seq.index st i) (Seq.index i_st i)
+    with i_s;
+
+    assert (not (has_slot tsm s));
+    assert (is_value_of root_key v);
+
+    let new_entry = {
+      key = root_key;
+      value = v;
+      add_method = MAdd;
+      l_child_in_store = None;
+      r_child_in_store = None;
+      parent_slot = None;
+    } in
+
+    let st_ = Seq.upd tsm.store (U16.v s) (Some new_entry) in
+    let tsm_ = madd_to_store_root tsm s v in
+    assert (tsm_.store == st_);
+
+    let i_st_ = IS.madd_to_store_root i_st i_s i_v in
+
+    let aux (i:_)
+      : Lemma (ensures (related_store_entry_opt (Seq.index st_ i) (Seq.index i_st_ i)))
+      = related_root_inv ();
+        if i <> i_s then
+        begin
+          assert (Seq.index st_ i == Seq.index st i);
+          assert (IS.identical_except i_st i_st_ i_s);
+
+          eliminate forall s'. s' <> i_s ==> IS.get_slot i_st s' = IS.get_slot i_st_ s'
+          with i
+        end
+    in
+    forall_intro aux;
+    ()
+
+let init_store_related (tid: AT.tid) (i_tid: i_tid)
+  : Lemma (requires (related_tid tid i_tid))
+          (ensures (let tsm = init_thread_state_model tid in
+                    let i_tsm = IV.init_thread_state i_vcfg i_tid in
+                    related_store tsm.store i_tsm.IV.st))
+  = let tsm = init_thread_state_model tid in
+    let st = tsm.store in
+    let i_st = IV.init_store i_vcfg i_tid in
+
+    let empty_st: TSM.contents = Seq.create (U16.v AT.store_size) None in
+    let i_empty_st = IS.empty_store i_vcfg in
+
+    empty_store_related ();
+    assert (related_store empty_st i_empty_st);
+
+    if i_tid = 0 then
+    begin
+
+      (* state of initial tsm before the madd *)
+      let _tsm = {
+        thread_id = tid;
+        failed = false;
+        store = Seq.create (U16.v AT.store_size) None;
+        clock = 0uL;
+        epoch_hashes = initial_epoch_hashes;
+        processed_entries = Seq.empty;
+        app_results = Seq.empty
+      } in
+
+      let s = U16.zero in
+      let i_s = 0 in
+      assert (related_slot s i_s);
+
+      let rk = root_key in
+      let v = init_value rk in
+
+      let i_rk: GK.key app = GK.IntK Zeta.BinTree.Root in
+      let i_v = R.init_value i_rk in
+
+      assert (related_val v i_v);
+
+      assert (tsm == madd_to_store_root _tsm U16.zero (init_value root_key));
+      related_madd_to_store_root _tsm i_empty_st s i_s v i_v;
+
+      ()
+    end
+    else
+    begin
+      assert (i_st == i_empty_st);
+      assert (st == empty_st);
+      ()
+    end
+
+let init_state_related (tid: AT.tid) (i_tid: i_tid)
+  : Lemma (requires (related_tid tid i_tid))
+          (ensures (let tsm = init_thread_state_model tid in
+                    let i_tsm = IV.init_thread_state i_vcfg i_tid in
+                    related_tsm tsm i_tsm))
+  = let tsm = init_thread_state_model tid in
+    let i_tsm = IV.init_thread_state i_vcfg i_tid in
+
+    // both models are in not failed state
+    assert (not tsm.failed /\ i_tsm.IV.valid);
+
+    // thread ids are equal by construction
+    assert (related_tid tsm.thread_id i_tsm.IV.tid);
+    related_timestamp_zero ();
+    assert (related_timestamp tsm.clock i_tsm.IV.clock);
+
+    init_store_related tid i_tid
+
+let init_tsm_spec_rel_base (tid: AT.tid)
+  : Lemma (ensures (spec_rel_base (init_thread_state_model tid)))
+  = let tsm = init_thread_state_model tid in
+    let i_tid = lift_tid tsm.thread_id in
+    init_state_related tid i_tid;
+    ()
+
+let length tsm = Seq.length tsm.processed_entries
+
+let prev (tsm: valid_tsm {length tsm > 0})
+  : thread_state_model
+  = let i = length tsm - 1 in
+    run tsm.thread_id (SA.prefix tsm.processed_entries i)
+
+let last_entry (tsm: valid_tsm {length tsm > 0})
+  : GTot (e:_ { valid_log_entry e })
+  = let i = length tsm - 1 in
+    Seq.index tsm.processed_entries i
+
+(* the prev of a valid tsm is also valid *)
+let valid_prev (tsm: valid_tsm {length tsm > 0} )
+  : Lemma (ensures (valid (prev tsm)))
+          [SMTPat (prev tsm)]
+  = let _tsm = prev tsm in
+    let e = last_entry tsm in
+
+    let l = tsm.processed_entries in
+    let i = length tsm - 1 in
+    let _l = SA.prefix l i in
+
+    // from definition of valid_tsm and run
+    assert (tsm == run tsm.thread_id tsm.processed_entries);
+    assert (tsm == verify_step_model _tsm e);
+
+    // from last assert, _tsm cannot be in failed state
+    assert (not _tsm.failed);
+
+    // definition of prev
+    assert (_tsm == run tsm.thread_id _l);
+
+    run_implies_processed_entries tsm.thread_id _l;
+    assert (_tsm.processed_entries == _l);
+
+    ()
+
+let lemma_prev_log_prefix (tsm: valid_tsm {length tsm > 0 })
+  : Lemma (ensures (let _tsm = prev tsm in
+                    let l = tsm.processed_entries in
+                    let i = length tsm - 1 in
+                    _tsm.processed_entries == SA.prefix l i))
+          [SMTPat (prev tsm)]
+  = let _tsm = prev tsm in
+    let e = last_entry tsm in
+
+    let l = tsm.processed_entries in
+    let i = Seq.length l - 1 in
+    let _l = SA.prefix l i in
+
+    // from definition of valid_tsm and run
+    assert (tsm == run tsm.thread_id tsm.processed_entries);
+    assert (tsm == verify_step_model _tsm e);
+
+    // from last assert, _tsm cannot be in failed state
+    assert (not _tsm.failed);
+
+    // definition of prev
+    assert (_tsm == run tsm.thread_id _l);
+
+    run_implies_processed_entries tsm.thread_id _l;
+    assert (_tsm.processed_entries == _l);
+
+    ()
+
+let spec_rel_base_snoc (tsm: valid_tsm {length tsm > 0})
+  : Lemma (requires (let _tsm = prev tsm in
+                     spec_rel_base _tsm))
+          (ensures (spec_rel_base tsm))
+  = let _tsm = prev tsm in
+    let e = last_entry tsm in
+    assert (tsm == verify_step_model _tsm e);
+    lemma_verify_step_model_spec_rel_base _tsm e
+
+let rec valid_implies_spec_rel_base (tsm: valid_tsm)
+  : Lemma (ensures (spec_rel_base tsm))
+          (decreases (length tsm))
+          [SMTPat (valid tsm)]
+  = let tid = tsm.thread_id in
+    let i_tid = lift_tid tid in
+    if length tsm = 0 then
+      init_tsm_spec_rel_base tid
+    else
+    begin
+      let _tsm = prev tsm in
+      valid_implies_spec_rel_base _tsm;
+      spec_rel_base_snoc tsm
+    end
+
+module GT = Zeta.Generic.Thread
+
+let init_add_set_empty (tsm: valid_tsm {length tsm = 0}) (ep: epoch_id)
+  : Lemma (ensures (add_set tsm (lift_epoch ep) == Zeta.MultiSet.empty))
+  = let i_ep = lift_epoch ep in
+    let tid = tsm.thread_id in
+    let l = tsm.processed_entries in
+
+    assert (tsm == init_thread_state_model tid);
+
+    let i_tl = to_ilog tsm in
+    assert (GT.length i_tl = 0);
+
+    let add_seq = GT.add_seq i_ep i_tl in
+
+    GT.add_seq_empty i_ep i_tl;
+    assert (Seq.length add_seq = 0);
+
+    let open Zeta.MultiSetHashDomain in
+    Zeta.MultiSet.zero_length_implies_empty #_ #(ms_hashfn_dom_cmp app) add_seq
+
+let init_hadd_correct (tsm: valid_tsm {length tsm = 0}) (ep: epoch_id)
+  : Lemma (ensures (let i_ep = lift_epoch ep in
+                    let eh = Map.sel tsm.epoch_hashes ep in
+                    eh.hadd = ms_hashfn (add_set tsm i_ep)))
+  = let i_ep = lift_epoch ep in
+    init_add_set_empty tsm ep;
+    lemma_hashfn_empty ();
+    assert (ms_hashfn (add_set tsm i_ep) == HA.initial_hash);
+    assert (tsm.epoch_hashes == initial_epoch_hashes);
+    ()
+
+let is_blum_add e =
+  let open T in
+  match e with
+  | AddB _ -> true
+  | AddBApp _ -> true
+  | _ -> false
+
+let blum_add_timestamp (e:_ {is_blum_add e})
+  = let open T in
+    match e with
+    | AddB p -> p.t
+    | AddBApp p -> p.t
+
+let blum_add_tid (e: _ {is_blum_add e})
+  = let open T in
+    match e with
+    | AddB p -> p.tid
+    | AddBApp p -> p.tid
+
+let blum_add_payload (e:_ {is_blum_add e})
+  = let open T in
+    match e with
+    | AddB p -> Inl (p.k, p.v)
+    | AddBApp p -> Inr p.rest
+
+let blum_add_slot (e:_ {is_blum_add e})
+  = let open T in
+    match e with
+    | AddB p -> p.s
+    | AddBApp p -> p.s
+
+let blum_add_record (e:_ {is_blum_add e})
+  = record_of_payload (blum_add_payload e)
+
+#push-options "--fuel 2 --ifuel 1 --z3rlimit_factor 3 --query_stats"
+
+let epoch_hashes_unchanged_addm (tsm: thread_state_model) (e: s_log_entry {T.AddM? e})
+  : Lemma (ensures (let tsm_ = verify_step_model tsm e in
+                    not tsm_.failed ==> tsm.epoch_hashes == tsm_.epoch_hashes))
+  = ()
+
+let epoch_hashes_unchanged_addmapp (tsm: thread_state_model) (e: s_log_entry {T.AddMApp? e})
+  : Lemma (ensures (let tsm_ = verify_step_model tsm e in
+                    not tsm_.failed ==> tsm.epoch_hashes == tsm_.epoch_hashes))
+  = ()
+
+let epoch_hashes_unchanged_evictm (tsm: thread_state_model) (e: s_log_entry {T.EvictM? e})
+  : Lemma (ensures (let tsm_ = verify_step_model tsm e in
+                    not tsm_.failed ==> tsm.epoch_hashes == tsm_.epoch_hashes))
+  = ()
+
+let epoch_hashes_unchanged_next_epoch (tsm: thread_state_model) (e: s_log_entry {T.NextEpoch? e})
+  : Lemma (ensures (let tsm_ = verify_step_model tsm e in
+                    not tsm_.failed ==> tsm.epoch_hashes == tsm_.epoch_hashes))
+  = ()
+
+let epoch_hashes_unchanged_verify_epoch
+    (tsm: thread_state_model)
+    (e: s_log_entry {T.VerifyEpoch? e})
+    (ep: epoch_id)
+  : Lemma (ensures (let tsm_ = verify_step_model tsm e in
+                    let eh = Map.sel tsm.epoch_hashes ep in
+                    let eh_ = Map.sel tsm_.epoch_hashes ep in
+                    not tsm_.failed ==> (eh.hadd == eh_.hadd /\
+                                         eh.hevict == eh_.hevict)))
+  = ()
+
+#pop-options
+
+let runapp_does_not_change_epoch_hashes (tsm: thread_state_model) (pl: T.runApp_payload)
+  : Lemma (ensures (let tsm_ = runapp tsm pl in
+                    not tsm_.failed ==> tsm_.epoch_hashes == tsm.epoch_hashes))
+  = let tsm_ = runapp tsm pl in
+    if not tsm_.failed then
+    begin
+      assert (Map.contains app.A.tbl pl.fid);
+      match AT.spec_app_parser pl.fid pl.rest.ebytes with
+      | Some ((arg, slots), len) ->
+        assert (len = U32.v pl.rest.len);
+        let fsig = Map.sel app.A.tbl pl.fid in
+        match read_slots tsm slots with
+        | Some recs ->
+          let res = fsig.f arg recs in
+          match res with
+          | (_, res, out_vals) ->
+            let tsm1 = {tsm with app_results=Seq.Properties.snoc tsm.app_results (| pl.fid, arg, recs, res |)} in
+            assert (tsm1.epoch_hashes == tsm.epoch_hashes);
+            assert (tsm_ == write_slots tsm1 slots out_vals);
+            write_slots_non_store_prop tsm1 slots out_vals;
+            assert (tsm_.epoch_hashes == tsm1.epoch_hashes);
+            ()
+    end
+
+let epoch_hashes_unchanged_runapp
+  (tsm: thread_state_model)
+  (e: s_log_entry {T.RunApp? e})
+  : Lemma (ensures (let tsm_ = verify_step_model tsm e in
+                    not tsm_.failed ==> tsm.epoch_hashes == tsm_.epoch_hashes))
+  = let T.RunApp p = e in
+    runapp_does_not_change_epoch_hashes tsm p
+
+let update_hadd_unchanged_hevict (tsm: thread_state_model)
+                                 (ep: epoch_id)
+                                 (r: T.record)
+                                 (t: T.timestamp)
+                                 (tid: T.thread_id)
+                                 (epi: epoch_id)
+  : Lemma (ensures (let tsm_ = update_hadd tsm ep r t tid in
+                    let eh = Map.sel tsm.epoch_hashes epi in
+                    let eh_ = Map.sel tsm.epoch_hashes epi in
+                    eh.hevict == eh_.hevict))
+  = ()
+
+let update_hevict_unchanged_hadd (tsm: thread_state_model)
+                                 (ep: epoch_id)
+                                 (r: T.record)
+                                 (t: T.timestamp)
+                                 (tid: T.thread_id)
+                                 (epi: epoch_id)
+  : Lemma (ensures (let tsm_ = update_hevict tsm ep r t tid in
+                    let eh = Map.sel tsm.epoch_hashes epi in
+                    let eh_ = Map.sel tsm.epoch_hashes epi in
+                    eh.hadd == eh_.hadd))
+  = ()
+
+let evict_hashes_unchanged_addb (tsm: thread_state_model) (e: s_log_entry {is_blum_add e}) (ep: epoch_id)
+  : Lemma (ensures (let tsm_ = verify_step_model tsm e in
+                    let eh = Map.sel tsm.epoch_hashes ep in
+                    let eh_ = Map.sel tsm_.epoch_hashes ep in
+                    not tsm_.failed ==> eh.hevict == eh_.hevict))
+  = let tsm_ = verify_step_model tsm e in
+    let eh = Map.sel tsm.epoch_hashes ep in
+    let eh_ = Map.sel tsm_.epoch_hashes ep in
+
+    let s = blum_add_slot e in
+    let t = blum_add_timestamp e in
+    let tid = blum_add_tid e in
+    let p = blum_add_payload e in
+
+    if not tsm_.failed then
+    begin
+      let Some (| k,v |) = record_of_payload p in
+      let tsm1 = update_hadd tsm (epoch_of_timestamp t) (k,v) t tid in
+      assert (tsm_.epoch_hashes == tsm1.epoch_hashes);
+      update_hadd_unchanged_hevict tsm (epoch_of_timestamp t) (k,v) t tid ep
+    end
+
+let add_hashes_unchanged_evictb (tsm: thread_state_model) (e: s_log_entry {T.EvictB? e}) (ep: epoch_id)
+  : Lemma (ensures (let tsm_ = verify_step_model tsm e in
+                    let eh = Map.sel tsm.epoch_hashes ep in
+                    let eh_ = Map.sel tsm_.epoch_hashes ep in
+                    not tsm_.failed ==> eh.hadd == eh_.hadd))
+  = ()
+
+let add_hashes_unchanged_evictbm (tsm: thread_state_model) (e: s_log_entry {T.EvictBM? e}) (ep: epoch_id)
+  : Lemma (ensures (let tsm_ = verify_step_model tsm e in
+                    let eh = Map.sel tsm.epoch_hashes ep in
+                    let eh_ = Map.sel tsm_.epoch_hashes ep in
+                    not tsm_.failed ==> eh.hadd == eh_.hadd))
+  = ()
+
+(* the add-set hashes remain unchanged with any operation other than addb/addbapp *)
+let add_hashes_unchanged_non_addb
+  (tsm: thread_state_model)
+  (e: s_log_entry {not (is_blum_add e)})
+  (ep: epoch_id)
+  : Lemma (ensures (let tsm_ = verify_step_model tsm e in
+                    let eh = Map.sel tsm.epoch_hashes ep in
+                    let eh_ = Map.sel tsm_.epoch_hashes ep in
+                    not tsm_.failed ==> eh.hadd == eh_.hadd))
+  = let open T in
+    match e with
+    | AddM _ -> epoch_hashes_unchanged_addm tsm e
+    | AddMApp _ -> epoch_hashes_unchanged_addmapp tsm e
+    | EvictM _ -> epoch_hashes_unchanged_evictm tsm e
+    | EvictB _ -> add_hashes_unchanged_evictb tsm e ep
+    | EvictBM _ -> add_hashes_unchanged_evictbm tsm e ep
+    | NextEpoch _ -> epoch_hashes_unchanged_next_epoch tsm e
+    | VerifyEpoch _ -> epoch_hashes_unchanged_verify_epoch tsm e ep
+    | RunApp _ -> epoch_hashes_unchanged_runapp tsm e
+
+let hadd_correct_snoc_non_addb (tsm: valid_tsm {length tsm > 0}) (ep: epoch_id)
+  : Lemma (requires (let i_ep = lift_epoch ep in
+                     let _tsm = prev tsm in
+                     let _eh = Map.sel _tsm.epoch_hashes ep in
+                     let e = last_entry tsm in
+                     not (is_blum_add e) /\
+                     _eh.hadd = ms_hashfn (add_set _tsm i_ep)))
+          (ensures (let i_ep = lift_epoch ep in
+                    let eh = Map.sel tsm.epoch_hashes ep in
+                    eh.hadd = ms_hashfn (add_set tsm i_ep)))
+  = let i = length tsm - 1 in
+    let e = last_entry tsm in
+    let eh = Map.sel tsm.epoch_hashes ep in
+
+    let _tsm = prev tsm in
+    let _eh = Map.sel _tsm.epoch_hashes ep in
+
+    // add hashes are unchanged for non-addb entries
+    add_hashes_unchanged_non_addb _tsm e ep;
+    assert (eh.hadd == _eh.hadd);
+
+    let i_ep = lift_epoch ep in
+    let i_e = lift_log_entry e in
+    let i_tl = to_ilog tsm in
+    let _i_tl = to_ilog _tsm in
+
+    // last entry is not a blum add in spec-level
+    assert (not (GT.is_blum_add_ep i_ep i_tl i));
+
+    // the add-seq remains unchanged
+    GT.add_seq_snoc i_ep  i_tl;
+    assert (GT.add_seq i_ep i_tl == GT.add_seq i_ep _i_tl);
+
+    ()
+
+let haddevict_unchanged_addb_diff_epoch
+  (tsm: thread_state_model)
+  (e: _ {is_blum_add e})
+  (ep: epoch_id)
+  : Lemma (requires (epoch_of_timestamp (blum_add_timestamp e) <> ep))
+          (ensures (let tsm_ = verify_step_model tsm e in
+                    let eh_ = Map.sel tsm_.epoch_hashes ep in
+                    let eh = Map.sel tsm.epoch_hashes ep in
+                    eh.hadd == eh_.hadd /\
+                    eh.hevict == eh_.hevict))
+  = ()
+
+let hadd_change_addb
+  (tsm: thread_state_model)
+  (e: _ {is_blum_add e})
+  (ep: epoch_id)
+  : Lemma (requires (epoch_of_timestamp (blum_add_timestamp e) = ep /\
+                     Some? (blum_add_record e)))
+          (ensures (let tsm_ = verify_step_model tsm e in
+                    let eh = Map.sel tsm.epoch_hashes ep in
+                    let eh_ = Map.sel tsm_.epoch_hashes ep in
+                    let Some (| k, v |) = blum_add_record e in
+                    let t = blum_add_timestamp e in
+                    let tid = blum_add_tid e in
+                    not tsm_.failed ==>
+                    eh_.hadd == update_hash_value eh.hadd (k,v) t tid))
+  = ()
+
+let hadd_correct_snoc_addb_diff_epoch (tsm: valid_tsm {length tsm > 0}) (ep: epoch_id)
+  : Lemma (requires (let i_ep = lift_epoch ep in
+                     let _tsm = prev tsm in
+                     let _eh = Map.sel _tsm.epoch_hashes ep in
+                     let e = last_entry tsm in
+                     is_blum_add e /\
+                     _eh.hadd = ms_hashfn (add_set _tsm i_ep) /\
+                     epoch_of_timestamp (blum_add_timestamp e) <> ep))
+          (ensures (let i_ep = lift_epoch ep in
+                    let eh = Map.sel tsm.epoch_hashes ep in
+                    eh.hadd = ms_hashfn (add_set tsm i_ep)))
+  = let i = length tsm - 1 in
+    let i_ep = lift_epoch ep in
+    let e = last_entry tsm in
+    let eh = Map.sel tsm.epoch_hashes ep in
+    let i_e = lift_log_entry e in
+    let i_tl = to_ilog tsm in
+
+    let i_tsm = to_i_tsm tsm in
+    assert (related_tsm tsm i_tsm);
+
+    let _tsm = prev tsm in
+    let _i_tsm = to_i_tsm _tsm in
+    let _eh = Map.sel _tsm.epoch_hashes ep in
+    let _i_tl = to_ilog _tsm in
+
+    assert (related_tsm _tsm _i_tsm);
+    assert (_i_tl == GT.prefix i_tl i);
+
+    let i_be = GT.blum_add_elem i_tl i in
+
+    let t = blum_add_timestamp e in
+    let tid = blum_add_tid e in
+    let Some (| k, v |) = blum_add_record e in
+    let s_be: s_dom =
+      let open Zeta.Steel.MultiSetHash in
+      { r = (k,v); t ; tid } in
+    assert (related_msdom s_be i_be);
+
+    let ep' = epoch_of_timestamp t in
+    assert (ep' <> ep);
+
+    assert (related_timestamp t i_be.t);
+    related_timestamp_epoch t i_be.t;
+
+    // since ep' <> ep, blum_add_seq is unchanged
+    GT.add_seq_snoc i_ep i_tl;
+    assert (GT.add_seq i_ep i_tl == GT.add_seq i_ep _i_tl);
+    assert (add_set tsm i_ep == add_set _tsm i_ep);
+
+    haddevict_unchanged_addb_diff_epoch _tsm e ep
+
+let hadd_correct_snoc_addb_same_epoch (tsm: valid_tsm {length tsm > 0}) (ep: epoch_id)
+  : Lemma (requires (let i_ep = lift_epoch ep in
+                     let _tsm = prev tsm in
+                     let _eh = Map.sel _tsm.epoch_hashes ep in
+                     let e = last_entry tsm in
+                     is_blum_add e /\
+                     _eh.hadd = ms_hashfn (add_set _tsm i_ep) /\
+                     epoch_of_timestamp (blum_add_timestamp e) = ep))
+          (ensures (let i_ep = lift_epoch ep in
+                    let eh = Map.sel tsm.epoch_hashes ep in
+                    eh.hadd = ms_hashfn (add_set tsm i_ep)))
+  = let i = length tsm - 1 in
+    let i_ep = lift_epoch ep in
+    let e = last_entry tsm in
+    let eh = Map.sel tsm.epoch_hashes ep in
+    let i_e = lift_log_entry e in
+    let i_tl = to_ilog tsm in
+
+    let i_tsm = to_i_tsm tsm in
+    assert (related_tsm tsm i_tsm);
+
+    let _tsm = prev tsm in
+    let _i_tsm = to_i_tsm _tsm in
+    let _eh = Map.sel _tsm.epoch_hashes ep in
+    let _i_tl = to_ilog _tsm in
+
+    assert (related_tsm _tsm _i_tsm);
+    assert (_i_tl == GT.prefix i_tl i);
+
+    let i_be = GT.blum_add_elem i_tl i in
+
+    let t = blum_add_timestamp e in
+    let tid = blum_add_tid e in
+    let Some (| k, v |) = blum_add_record e in
+    let s_be: s_dom =
+      let open Zeta.Steel.MultiSetHash in
+      { r = (k,v); t ; tid } in
+    assert (related_msdom s_be i_be);
+
+    assert (related_timestamp t i_be.t);
+    related_timestamp_epoch t i_be.t;
+
+    GT.add_seq_snoc i_ep i_tl;
+    assert (GT.is_blum_add_ep i_ep i_tl i);
+
+    assert (GT.add_seq i_ep i_tl == SA.append1 (GT.add_seq i_ep _i_tl) i_be);
+    let open Zeta.MultiSetHashDomain in
+    Zeta.MultiSet.seq2mset_add_elem #_ #(ms_hashfn_dom_cmp app) (GT.add_seq i_ep _i_tl) i_be;
+    assert (add_set tsm i_ep == MS.add_elem (add_set _tsm i_ep) i_be);
+
+    hadd_change_addb _tsm e ep;
+    lemma_update (add_set _tsm i_ep) i_be s_be;
+    ()
+
+let hadd_correct_snoc (tsm: valid_tsm {length tsm > 0}) (ep: epoch_id)
+  : Lemma (requires (let i_ep = lift_epoch ep in
+                     let _tsm = prev tsm in
+                     let _eh = Map.sel _tsm.epoch_hashes ep in
+                     _eh.hadd = ms_hashfn (add_set _tsm i_ep)))
+          (ensures (let i_ep = lift_epoch ep in
+                    let eh = Map.sel tsm.epoch_hashes ep in
+                    eh.hadd = ms_hashfn (add_set tsm i_ep)))
+  = let e = last_entry tsm in
+
+    if is_blum_add e then
+      if epoch_of_timestamp (blum_add_timestamp e) = ep then
+        hadd_correct_snoc_addb_same_epoch tsm ep
+      else
+        hadd_correct_snoc_addb_diff_epoch tsm ep
+    else
+      hadd_correct_snoc_non_addb tsm ep
+
+let rec valid_implies_hadd_correct (tsm: valid_tsm) (ep: epoch_id)
+  : Lemma (ensures (let i_ep = lift_epoch ep in
+                    let eh = Map.sel tsm.epoch_hashes ep in
+                    eh.hadd = ms_hashfn (add_set tsm i_ep)))
+          (decreases (length tsm))
+  = if length tsm = 0 then
+      init_hadd_correct tsm ep
+    else
+    begin
+      let _tsm = prev tsm in
+      valid_implies_hadd_correct _tsm ep;
+      hadd_correct_snoc tsm ep
+    end
+
+let init_evict_set_empty (tsm: valid_tsm {length tsm = 0}) (ep: epoch_id)
+  : Lemma (ensures (evict_set tsm (lift_epoch ep) == Zeta.MultiSet.empty))
+  = let i_ep = lift_epoch ep in
+    let tid = tsm.thread_id in
+    let l = tsm.processed_entries in
+
+    assert (tsm == init_thread_state_model tid);
+
+    let i_tl = to_ilog tsm in
+    assert (GT.length i_tl = 0);
+
+    let evict_seq = GT.evict_seq i_ep i_tl in
+    GT.evict_seq_empty i_ep i_tl;
+    assert (Seq.length evict_seq = 0);
+
+    let open Zeta.MultiSetHashDomain in
+    Zeta.MultiSet.zero_length_implies_empty #_ #(ms_hashfn_dom_cmp app) evict_seq
+
+let init_hevict_correct (tsm: valid_tsm {length tsm = 0}) (ep: epoch_id)
+  : Lemma (ensures (let i_ep = lift_epoch ep in
+                    let eh = Map.sel tsm.epoch_hashes ep in
+                    eh.hevict = ms_hashfn (evict_set tsm i_ep)))
+  = let i_ep = lift_epoch ep in
+    init_evict_set_empty tsm ep;
+    lemma_hashfn_empty ();
+    ()
+
+let is_blum_evict e =
+  let open T in
+  match e with
+  | EvictB _ -> true
+  | EvictBM _ -> true
+  | _ -> false
+
+let blum_evict_timestamp (e:_ {is_blum_evict e})
+  = let open T in
+    match e with
+    | EvictB p -> p.t
+    | EvictBM p -> p.t
+
+let blum_evict_slot (e:_ {is_blum_evict e})
+  = let open T in
+    match e with
+    | EvictB p -> p.s
+    | EvictBM p -> p.s
+
+let evict_hashes_unchanged_non_evict
+  (tsm: thread_state_model)
+  (e: s_log_entry { not (is_blum_evict e) })
+  (ep: epoch_id)
+  : Lemma (ensures (let tsm_ = verify_step_model tsm e in
+                    let eh = Map.sel tsm.epoch_hashes ep in
+                    let eh_ = Map.sel tsm_.epoch_hashes ep in
+                    not tsm_.failed ==> eh.hevict == eh_.hevict))
+  = let open T in
+    match e with
+    | AddM _ -> epoch_hashes_unchanged_addm tsm e
+    | AddMApp _ -> epoch_hashes_unchanged_addmapp tsm e
+    | AddB _ -> evict_hashes_unchanged_addb tsm e ep
+    | AddBApp _ -> evict_hashes_unchanged_addb tsm e ep
+    | EvictM _ -> epoch_hashes_unchanged_evictm tsm e
+    | NextEpoch _ -> epoch_hashes_unchanged_next_epoch tsm e
+    | VerifyEpoch _ -> epoch_hashes_unchanged_verify_epoch tsm e ep
+    | RunApp _ -> epoch_hashes_unchanged_runapp tsm e
+
+let hevict_change_evictb
+  (tsm: thread_state_model)
+  (e:_ {T.EvictB? e \/ T.EvictBM? e})
+  : Lemma (requires (let s = blum_evict_slot e in
+                     let t = blum_evict_timestamp e in
+                     check_slot_bounds s /\
+                     sat_evictb_checks tsm s t))
+          (ensures (let s = blum_evict_slot e in
+                    let t = blum_evict_timestamp e in
+                    let ep = epoch_of_timestamp t in
+                    let eh = Map.sel tsm.epoch_hashes ep in
+                    let Some r = get_entry tsm s in
+                    let tsm_ = verify_step_model tsm e in
+                    let eh_ = Map.sel tsm_.epoch_hashes ep in
+                    not tsm_.failed ==>
+                    eh_.hevict == update_hash_value eh.hevict (r.key, r.value) t tsm.thread_id))
+  = ()
+
+let hevict_correct_snoc_non_evictb
+  (tsm: valid_tsm {length tsm > 0}) (ep: epoch_id)
+  : Lemma (requires (let i_ep = lift_epoch ep in
+                     let _tsm = prev tsm in
+                     let _eh = Map.sel _tsm.epoch_hashes ep in
+                     let e = last_entry tsm in
+                     not (is_blum_evict e) /\
+                     _eh.hevict = ms_hashfn (evict_set _tsm i_ep)))
+          (ensures (let i_ep = lift_epoch ep in
+                    let eh = Map.sel tsm.epoch_hashes ep in
+                    eh.hevict = ms_hashfn (evict_set tsm i_ep)))
+  = let i = length tsm - 1 in
+    let e = last_entry tsm in
+    let eh = Map.sel tsm.epoch_hashes ep in
+
+    let _tsm = prev tsm in
+    let _eh = Map.sel _tsm.epoch_hashes ep in
+
+    evict_hashes_unchanged_non_evict _tsm e ep;
+    assert (eh.hevict == _eh.hevict);
+
+    let i_ep = lift_epoch ep in
+    let i_e = lift_log_entry e in
+    let i_tl = to_ilog tsm in
+    let _i_tl = to_ilog _tsm in
+
+    assert (not (GT.is_blum_evict_ep i_ep i_tl i));
+
+    GT.evict_seq_snoc i_ep i_tl;
+    assert (GT.evict_seq i_ep i_tl == GT.evict_seq i_ep _i_tl);
+    ()
+
+module MSD = Zeta.MultiSetHashDomain
+
+let blum_evict_elem (tsm: valid_tsm {length tsm > 0 /\ is_blum_evict (last_entry tsm)})
+  : GTot (Zeta.Steel.MultiSetHash.s_dom)
+  = let i = length tsm - 1 in
+    let e = last_entry tsm in
+    let s = blum_evict_slot e in
+    let t = blum_evict_timestamp e in
+    let _tsm = prev tsm in
+    let Some r0 = get_entry _tsm s in
+    let r = (r0.key, r0.value) in
+    let s_be: s_dom =
+      let open Zeta.Steel.MultiSetHash in
+      { r ; t; tid = tsm.thread_id } in
+    s_be
+
+#push-options "--fuel 1 --ifuel 1 --z3rlimit_factor 3 --query_stats"
+
+let related_blum_evict_elem (tsm: valid_tsm {spec_rel_base tsm /\ length tsm > 0})
+  : Lemma (requires (is_blum_evict (last_entry tsm)))
+          (ensures (let i = length tsm - 1 in
+                    let i_tl = to_ilog tsm in
+                    let i_be = GT.blum_evict_elem i_tl i in
+                    let s_be = blum_evict_elem tsm in
+                    Zeta.Steel.MultiSetHash.related_msdom s_be i_be))
+  = let i = length tsm - 1 in
+    let e = last_entry tsm in
+    let i_tl = to_ilog tsm in
+    let i_be = GT.blum_evict_elem i_tl i in
+    let s_be = blum_evict_elem tsm in
+
+    let _tsm = prev tsm in
+    let _st = _tsm.store in
+
+    let _i_tsm = to_i_tsm _tsm in
+    let _i_st = _i_tsm.IV.st in
+    assert (related_store _st _i_st);
+
+    let MSD.MHDom i_r i_t i_j = i_be in
+
+    let s = blum_evict_slot e in
+
+    let Some se = get_slot _st s in
+    assert (s_be.r = (se.key, se.value));
+
+    let i_e = GT.index i_tl i in
+    let i_s = GV.evict_slot i_e in
+    assert (related_log_entry e i_e);
+    assert (related_slot s i_s);
+
+    eliminate forall i. related_store_entry_opt (Seq.index _st i) (Seq.index _i_st i)
+    with i_s;
+
+    let Some ie = Seq.index _i_st i_s in
+    assert (related_store_entry_opt (Some se) (Some ie));
+    assert (related_store_entry se ie);
+    let IS.VStoreE i_r2 _ _ _ _ = ie in
+
+    assert (related_record (se.key, se.value) i_r2);
+    assert (related_record s_be.r i_r2);
+    assert (i_r2 = i_r);
+    ()
+
+#pop-options
+
+#push-options "--fuel 1 --ifuel 1 --query_stats"
+
+let hevict_correct_snoc_evictb_same_epoch
+  (tsm: valid_tsm {length tsm > 0})
+  (ep: epoch_id)
+  : Lemma (requires (let i_ep = lift_epoch ep in
+                     let _tsm = prev tsm in
+                     let _eh = Map.sel _tsm.epoch_hashes ep in
+                     let e = last_entry tsm in
+                     is_blum_evict e /\
+                     _eh.hevict = ms_hashfn (evict_set _tsm i_ep) /\
+                     epoch_of_timestamp (blum_evict_timestamp e) = ep))
+           (ensures (let i_ep = lift_epoch ep in
+                     let eh = Map.sel tsm.epoch_hashes ep in
+                     eh.hevict = ms_hashfn (evict_set tsm i_ep)))
+ = let i = length tsm - 1 in
+   let i_ep = lift_epoch ep in
+   let e = last_entry tsm in
+   let eh = Map.sel tsm.epoch_hashes ep in
+   let i_e = lift_log_entry e in
+
+   let i_tl = to_ilog tsm in
+   let i_tsm = to_i_tsm tsm in
+   assert (related_tsm tsm i_tsm);
+
+   let _tsm = prev tsm in
+   let _i_tsm = to_i_tsm _tsm in
+   let _eh = Map.sel _tsm.epoch_hashes ep in
+   let _i_tl = to_ilog _tsm in
+   assert (related_tsm _tsm _i_tsm);
+   assert (_i_tl = GT.prefix i_tl i);
+
+   let i_be = GT.blum_evict_elem i_tl i in
+   let t = blum_evict_timestamp e in
+   let tid = tsm.thread_id in
+   let s = blum_evict_slot e in
+   let i_s = lift_slot s in
+   assert (i_s = GV.evict_slot i_e);
+
+   assert (tsm == verify_step_model _tsm e);
+
+   let s_be = blum_evict_elem tsm in
+
+   let MSD.MHDom i_r i_t i_j = i_be in
+   related_blum_evict_elem tsm;
+   related_timestamp_epoch t i_t;
+   assert (GT.is_blum_evict_ep i_ep i_tl i);
+   GT.evict_seq_snoc i_ep i_tl;
+
+   assert (GT.evict_seq i_ep i_tl == SA.append1 (GT.evict_seq i_ep _i_tl) i_be);
+   let open Zeta.MultiSetHashDomain in
+   Zeta.MultiSet.seq2mset_add_elem #_ #(ms_hashfn_dom_cmp app) (GT.evict_seq i_ep _i_tl) i_be;
+   assert (evict_set tsm i_ep == MS.add_elem (evict_set _tsm i_ep) i_be);
+
+   hevict_change_evictb _tsm e;
+   lemma_update (evict_set _tsm i_ep) i_be s_be;
+   ()
+
+#pop-options
+
+let haddevict_unchanged_evictb_diff_epoch
+  (tsm: thread_state_model)
+  (e: _ {is_blum_evict e})
+  (ep: epoch_id)
+  : Lemma (requires (epoch_of_timestamp (blum_evict_timestamp e) <> ep))
+          (ensures (let tsm_ = verify_step_model tsm e in
+                    let eh_ = Map.sel tsm_.epoch_hashes ep in
+                    let eh = Map.sel tsm.epoch_hashes ep in
+                    eh.hadd == eh_.hadd /\
+                    eh.hevict == eh_.hevict))
+  = ()
+
+#push-options "--fuel 1 --ifuel 1 --query_stats"
+
+let hevict_correct_snoc_evictb_diff_epoch (tsm: valid_tsm {length tsm > 0}) (ep: epoch_id)
+  : Lemma (requires (let i_ep = lift_epoch ep in
+                     let _tsm = prev tsm in
+                     let _eh = Map.sel _tsm.epoch_hashes ep in
+                     let e = last_entry tsm in
+                     is_blum_evict e /\
+                     _eh.hevict = ms_hashfn (evict_set _tsm i_ep) /\
+                     epoch_of_timestamp (blum_evict_timestamp e) <> ep))
+          (ensures (let i_ep = lift_epoch ep in
+                    let eh = Map.sel tsm.epoch_hashes ep in
+                    eh.hevict = ms_hashfn (evict_set tsm i_ep)))
+  = let i = length tsm - 1 in
+    let i_ep = lift_epoch ep in
+    let e = last_entry tsm in
+    let eh = Map.sel tsm.epoch_hashes ep in
+
+    let i_e = lift_log_entry e in
+    let i_tl = to_ilog tsm in
+    let i_tsm = to_i_tsm tsm in
+    assert (related_tsm tsm i_tsm);
+
+    let _tsm = prev tsm in
+    let _i_tsm = to_i_tsm _tsm in
+    let _eh = Map.sel _tsm.epoch_hashes ep in
+    let _i_tl = to_ilog _tsm in
+
+    assert (related_tsm _tsm _i_tsm);
+    assert (_i_tl == GT.prefix i_tl i);
+    assert (i_e = GT.index i_tl i);
+
+    assert (GT.is_blum_evict i_tl i);
+    let i_be = GT.blum_evict_elem i_tl i in
+    let t = blum_evict_timestamp e in
+    let ep' = epoch_of_timestamp t in
+    assert (ep <> ep');
+
+    assert (related_timestamp t i_be.MSD.t);
+    related_timestamp_epoch t i_be.MSD.t;
+
+    assert (~ (GT.is_blum_evict_ep i_ep i_tl i));
+    GT.evict_seq_snoc i_ep i_tl;
+    assert (GT.evict_seq i_ep i_tl == GT.evict_seq i_ep _i_tl);
+    assert (evict_set tsm i_ep == evict_set _tsm i_ep);
+
+    haddevict_unchanged_evictb_diff_epoch _tsm e ep
+
+#pop-options
+
+let hevict_correct_snoc (tsm: valid_tsm {length tsm > 0}) (ep: epoch_id)
+  : Lemma (requires (let i_ep = lift_epoch ep in
+                     let _tsm = prev tsm in
+                     let _eh = Map.sel _tsm.epoch_hashes ep in
+                     _eh.hevict = ms_hashfn (evict_set _tsm i_ep)))
+          (ensures (let i_ep = lift_epoch ep in
+                    let eh = Map.sel tsm.epoch_hashes ep in
+                    eh.hevict = ms_hashfn (evict_set tsm i_ep)))
+  = let e = last_entry tsm in
+
+    if is_blum_evict e then
+      if epoch_of_timestamp (blum_evict_timestamp e) = ep then
+        hevict_correct_snoc_evictb_same_epoch tsm ep
+      else
+        hevict_correct_snoc_evictb_diff_epoch tsm ep
+    else
+      hevict_correct_snoc_non_evictb tsm ep
+
+let rec valid_implies_hevict_correct (tsm: valid_tsm) (ep: epoch_id)
+  : Lemma (ensures (let i_ep = lift_epoch ep in
+                    let eh = Map.sel tsm.epoch_hashes ep in
+                    eh.hevict = ms_hashfn (evict_set tsm i_ep)))
+          (decreases (length tsm))
+  = if length tsm = 0 then
+      init_hevict_correct tsm ep
+    else
+    begin
+      let _tsm = prev tsm in
+      valid_implies_hevict_correct _tsm ep;
+      hevict_correct_snoc tsm ep
+    end
+
+let valid_implies_epoch_hashes_correct (tsm: valid_tsm)
+  : Lemma (ensures (forall (ep: epoch_id). let i_ep = lift_epoch ep in
+                                      let eh = Map.sel tsm.epoch_hashes ep in
+                                      eh.hadd = ms_hashfn (add_set tsm i_ep) /\
+                                      eh.hevict = ms_hashfn (evict_set tsm i_ep)))
+  = let aux (ep:_)
+      : Lemma (ensures (let i_ep = lift_epoch ep in
+                        let eh = Map.sel tsm.epoch_hashes ep in
+                        eh.hadd = ms_hashfn (add_set tsm i_ep) /\
+                        eh.hevict = ms_hashfn (evict_set tsm i_ep)))
+      = let i_ep = lift_epoch ep in
+        let eh = Map.sel tsm.epoch_hashes ep in
+        valid_implies_hadd_correct tsm ep;
+        valid_implies_hevict_correct tsm ep
+    in
+    forall_intro aux
+
+let valid_implies_spec_rel (tsm: valid_tsm)
+  : Lemma (ensures (spec_rel tsm))
+  = valid_implies_epoch_hashes_correct tsm
+
+let valid_hadd_prop (ep: TSM.epoch_id) (tsm: valid_tsm)
+  : Lemma (ensures (let i_ep = lift_epoch ep in
+                    let eh = Map.sel tsm.epoch_hashes ep in
+                    eh.hadd = ms_hashfn (add_set tsm i_ep)))
+  = valid_implies_epoch_hashes_correct tsm;
+    eliminate forall (ep: epoch_id). let i_ep = lift_epoch ep in
+                                let eh = Map.sel tsm.epoch_hashes ep in
+                                eh.hadd = ms_hashfn (add_set tsm i_ep) /\
+                                eh.hevict = ms_hashfn (evict_set tsm i_ep)
+    with ep;
+    ()
+
+let valid_hevict_prop (ep: TSM.epoch_id) (tsm: valid_tsm)
+  : Lemma (ensures (let i_ep = lift_epoch ep in
+                    let eh = Map.sel tsm.epoch_hashes ep in
+                    eh.hevict = ms_hashfn (evict_set tsm i_ep)))
+  = valid_implies_epoch_hashes_correct tsm;
+    eliminate forall (ep: epoch_id). let i_ep = lift_epoch ep in
+                                let eh = Map.sel tsm.epoch_hashes ep in
+                                eh.hadd = ms_hashfn (add_set tsm i_ep) /\
+                                eh.hevict = ms_hashfn (evict_set tsm i_ep)
+    with ep;
+    ()
+
+let run_props (tid: AT.tid) (l: s_log)
+  : Lemma (ensures (let tsm = run tid l in
+                    (not tsm.failed) ==> (valid tsm /\
+                                         tsm.thread_id = tid /\
+                                         tsm.processed_entries == l)))
+  = run_implies_thread_id tid l;
+    run_implies_processed_entries tid l;
+    run_implies_valid tid l
