steel/Zeta.Steel.ThreadRel.fsti
@@ -1,0 +1,109 @@
+module Zeta.Steel.ThreadRel
+
+(* This module sets up the relationship between a steel verifier thread and a spec-level one *)
+
+open Zeta.App
+open Zeta.AppSimulate
+open Zeta.Steel.KeyUtils
+open Zeta.Steel.Rel
+open Zeta.Steel.LogRel
+open Zeta.Steel.StoreRel
+open Zeta.Steel.MultiSetHash
+open Zeta.Steel.ThreadStateModel
+open Zeta.Steel.ThreadRelDef
+
+module U8 = FStar.UInt8
+module U16 = FStar.UInt16
+module U32 = FStar.UInt32
+module L = FStar.List.Tot
+module GK = Zeta.GenKey
+module K = Zeta.Key
+module M = Zeta.Merkle
+module GV = Zeta.GenericVerifier
+module GT = Zeta.Generic.Thread
+module IL = Zeta.Intermediate.Logs
+module IV = Zeta.Intermediate.Verifier
+module AT = Zeta.Steel.ApplicationTypes
+module T = Zeta.Steel.FormatsManual
+module TSM = Zeta.Steel.ThreadStateModel
+module MS = Zeta.MultiSet
+
+(* thread_state_model has some redundancy - for tsm's of interest, the state is obtained by
+ * running the log from an initial state. *)
+let valid (tsm: thread_state_model)
+  = U16.v tsm.thread_id < U32.v AT.n_threads /\
+    tsm == run tsm.thread_id tsm.processed_entries /\
+    not tsm.failed
+
+(* this type captures the class of well-behaved tsms we are interested in *)
+let valid_tsm = tsm: thread_state_model { valid tsm }
+
+(* the processed_entries of a valid tsm is a valid log - otherwise, the verify_step should have failed ... *)
+val valid_implies_valid_log (tsm: valid_tsm)
+  : Lemma (ensures (valid_log tsm.processed_entries))
+          [SMTPat (valid_log tsm.processed_entries)]
+
+
+let related_tsm_valid (s: s_thread_state) (i: i_thread_state)
+  = related_tsm s i /\
+    not s.failed
+
+(* tsm and its lifted spec version are related in all fields except epoch_hashes .... *)
+let spec_rel_base (tsm: valid_tsm)
+  = let open Zeta.Generic.Thread in
+    let open IV in
+    let open TSM in
+    let i_log = lift_log tsm.processed_entries in
+    let i_tid = lift_tid tsm.thread_id in
+    let i_tl = (i_tid, i_log) in
+    let i_tsm = state i_tl in
+
+    related_tsm tsm i_tsm
+
+let i_verifiable_log = Zeta.Intermediate.Thread.verifiable_log i_vcfg
+
+let to_ilog (tsm: valid_tsm {spec_rel_base tsm})
+  : GTot i_verifiable_log
+  = let i_log = lift_log tsm.processed_entries in
+    let i_tid = lift_tid tsm.thread_id in
+    (i_tid, i_log)
+
+let add_set (tsm: valid_tsm {spec_rel_base tsm}) (ep: i_epoch)
+  : GTot mset
+  = let tl = to_ilog tsm in
+    let add_seq = Zeta.Generic.Thread.add_seq ep tl in
+    MS.seq2mset add_seq
+
+let evict_set (tsm: valid_tsm {spec_rel_base tsm}) (ep: i_epoch)
+  : GTot mset
+  = let tl = to_ilog tsm in
+    let evict_seq = Zeta.Generic.Thread.evict_seq ep tl in
+    MS.seq2mset evict_seq
+
+(* spec_rel_base plus the epoch hashes are related to the add/evict sets *)
+let spec_rel (tsm: valid_tsm)
+  = spec_rel_base tsm /\
+    (forall (s_ep: epoch_id). let i_ep = lift_epoch s_ep in
+                          let eh = Map.sel tsm.epoch_hashes s_ep in
+                          eh.hadd = ms_hashfn (add_set tsm i_ep) /\
+                          eh.hevict = ms_hashfn (evict_set tsm i_ep))
+
+val valid_implies_spec_rel (tsm: valid_tsm)
+  : Lemma (ensures (spec_rel tsm))
+          [SMTPat (valid tsm)]
+
+val valid_hadd_prop (ep: TSM.epoch_id) (tsm: valid_tsm)
+  : Lemma (ensures (let i_ep = lift_epoch ep in
+                    let eh = Map.sel tsm.epoch_hashes ep in
+                    eh.hadd = ms_hashfn (add_set tsm i_ep)))
+
+val valid_hevict_prop (ep: TSM.epoch_id) (tsm: valid_tsm)
+  : Lemma (ensures (let i_ep = lift_epoch ep in
+                    let eh = Map.sel tsm.epoch_hashes ep in
+                    eh.hevict = ms_hashfn (evict_set tsm i_ep)))
+
+val run_props (tid: AT.tid) (l: s_log)
+  : Lemma (ensures (let tsm = run tid l in
+                    (not tsm.failed) ==> (valid tsm /\
+                                         tsm.thread_id = tid /\
+                                         tsm.processed_entries == l)))
