steel/Zeta.Steel.ThreadRelDef.fst
@@ -1,0 +1,16 @@
+module Zeta.Steel.ThreadRelDef
+
+(* This module defines related_tsm - the thread state (tsm) is related at steel layer and intermediate
+ * layer. *)
+
+open Zeta.Steel.Rel
+open Zeta.Steel.StoreRel
+
+module IV = Zeta.Intermediate.Verifier
+
+let related_tsm (s: s_thread_state) (i: i_thread_state)
+  = (not s.failed = i.IV.valid) /\
+    (i.IV.valid ==>
+     ((related_tid s.thread_id i.IV.tid) /\
+      (related_timestamp s.clock i.IV.clock) /\
+      (related_store s.store i.IV.st)))
